Format terms.v

B_Unification/terms.v
@@ -14,32 +14,31 @@ Require Import Setoid.
 Import ListNotations.
 
 (** * Introduction **)
-(**
-In order for any proofs to be constructed in Coq, we need to formally define the logic
-and data across which said proofs will operate. Since the heart of our analysis is 
-concerned with the unification of Boolean equations, it stands to reason that we should
-articulate precisely how algebra functions with respect to Boolean rings. To attain this,
-we shall formalize what an equation looks like, how it can be composed inductively, and also
-how substitutions behave when applied to equations.
-**)
+
+(** In order for any proofs to be constructed in Coq, we need to formally define
+    the logic and data across which said proofs will operate. Since the heart of
+    our analysis is concerned with the unification of Boolean equations, it
+    stands to reason that we should articulate precisely how algebra functions
+    with respect to Boolean rings. To attain this, we shall formalize what an
+    equation looks like, how it can be composed inductively, and also how
+    substitutions behave when applied to equations. *)
 
 (** * Terms **)
 
 (** ** Definitions **)
-(**
-We shall now begin describing the rules of Boolean arithmetic as well as the nature
-of Boolean equations. For simplicity's sake, from now on we shall be referring to equations 
-as terms.
-**)
 
-(* Define a variable to be a natural number *)
+(** We shall now begin describing the rules of Boolean arithmetic as well as the
+    nature of Boolean equations. For simplicity's sake, from now on we shall be
+    referring to equations as terms. *)
+
+(*  Define a variable to be a natural number *)
 Definition var := nat.
 
 Definition var_eq_dec := Nat.eq_dec.
 
-(**
-A term, as has already been previously described, is now inductively declared to hold either a constant value, a single variable, a sum of terms, or a product of terms.
-**)
+(** A _term_, as has already been previously described, is now inductively
+    declared to hold either a constant value, a single variable, a sum of terms,
+    or a product of terms. *)
 
 Inductive term: Type :=
   | T0  : term
@@ -48,9 +47,8 @@ Inductive term: Type :=
   | SUM : term -> term -> term
   | PRODUCT : term -> term -> term.
 
-(**
-For convenience's sake, we define some shorthanded notation for readability.
-**)
+(** For convenience's sake, we define some shorthanded notation for readability.
+    *)
 
 Implicit Types x y z : term.
 Implicit Types n m : var.
@@ -60,54 +58,59 @@ Notation "x * y" := (PRODUCT x y) (at level 40, left associativity).
 
 (** ** Axioms *)
 
-(** 
-Now that we have informed Coq on the nature of what a term is, it is now time to propose a set of axioms that will articulate exactly how algebra behaves across Boolean rings. This is
-a requirement since the very act of unifying an equation is intimately related to solving it algebraically. Each of the axioms proposed below describe the rules of Boolean algebra
-precisely and in an unambiguous manner. None of these should come as a surprise to the reader; however, if one is not familiar with this form of logic, the rules regarding the
-summation and multiplication of identical terms might pose as a source of confusion. 
+(** Now that we have informed Coq on the nature of what a term is, it is now
+    time to propose a set of axioms that will articulate exactly how algebra
+    behaves across Boolean rings. This is a requirement since the very act of
+    unifying an equation is intimately related to solving it algebraically. Each
+    of the axioms proposed below describe the rules of Boolean algebra precisely
+    and in an unambiguous manner. None of these should come as a surprise to the
+    reader; however, if one is not familiar with this form of logic, the rules
+    regarding the summation and multiplication of identical terms might pose as
+    a source of confusion.
 
-For reasons of keeping Coq's internal logic consistent, we roll our own custom equivalence relation as opposed to simply using '='. This will provide a surefire way to avoid any
-odd errors from later cropping up in our proofs. Of course, by doing this we introduce some implications that we will need to address later.
-**)
+    For reasons of keeping Coq's internal logic consistent, we roll our own
+    custom equivalence relation as opposed to simply using "=". This will
+    provide a surefire way to avoid any odd errors from later cropping up in our
+    proofs. Of course, by doing this we introduce some implications that we will
+    need to address later. *)
 
 Parameter eqv : term -> term -> Prop.
-(* Notation for term equivalence *)
+(*  Notation for term equivalence *)
 Infix " == " := eqv (at level 70).
 
-(* Commutatitivty across summations *)
+(*  Commutatitivty across summations *)
 Axiom sum_comm : forall x y, x + y == y + x.
 
-(* Associativity across summations *)
+(*  Associativity across summations *)
 Axiom sum_assoc : forall x y z, (x + y) + z == x + (y + z).
 
-(* Identity relation accross summations *)
+(*  Identity relation accross summations *)
 Axiom sum_id : forall x, T0 + x == x. 
 
-(* Across boolean rings, summation x + x will always be 0 because x can only be 0 or 1*)
+(*  Across boolean rings, summation x + x will always be 0 because x can only be
+   0 or 1*)
 Axiom sum_x_x : forall x, x + x == T0.
 
-(* Commutativity across multiplications *)
+(*  Commutativity across multiplications *)
 Axiom mul_comm : forall x y, x * y == y * x.
 
-(* Associativity across multiplications *)
+(*  Associativity across multiplications *)
 Axiom mul_assoc : forall x y z, (x * y) * z == x * (y * z).
 
-(* Across bollean rings, x * x will always be x because x can only be 0 or 1 *)
+(*  Across bollean rings, x * x will always be x because x can only be 0 or 1 *)
 Axiom mul_x_x : forall x, x * x == x.
 
-(* Multiplying anything by 0 is 0*)
+(*  Multiplying anything by 0 is 0*)
 Axiom mul_T0_x : forall x, T0 * x == T0.
 
-(* Identity relation across multiplications *)
+(*  Identity relation across multiplications *)
 Axiom mul_id : forall x, T1 * x == x.
 
-(* Distributivity relation *)
+(*  Distributivity relation *)
 Axiom distr : forall x y z, x * (y + z) == (x * y) + (x * z).
 
-(* 
-   Across all equations, adding an expression to both sides does not 
-   break the equivalence of the relation 
-*)
+(*  Across all equations, adding an expression to both sides does not
+   break the equivalence of the relation *)
 Axiom term_sum_symmetric :
   forall x y z, x == y <-> x + z == y + z.
 
@@ -120,12 +123,12 @@ Axiom T1_not_equiv_T0 :
 Hint Resolve sum_comm sum_assoc sum_x_x sum_id distr
              mul_comm mul_assoc mul_x_x mul_T0_x mul_id.
 
-(**
-Now that the core axioms have been taken care of, we need to handle the implications posed by our custom equivalence relation. Below we inform Coq of the behavior of our
-equivalence relation with respect to rewrites during proofs.
-**)
+(** Now that the core axioms have been taken care of, we need to handle the
+    implications posed by our custom equivalence relation. Below we inform Coq
+    of the behavior of our equivalence relation with respect to rewrites during
+    proofs. *)
 
-(* Mundane coq magic for custom equivalence relation *)
+(*  Mundane coq magic for custom equivalence relation *)
 Axiom eqv_ref : Reflexive eqv.
 Axiom eqv_sym : Symmetric eqv.
 Axiom eqv_trans : Transitive eqv.
@@ -162,57 +165,57 @@ Hint Resolve eqv_ref eqv_sym eqv_trans SUM_compat PRODUCT_compat.
 
 (** ** Lemmas **)
 
-(**
-Since Coq now understands the basics of Boolean algebra, it serves as a good exercise for us to generate some further rules using Coq's proving systems. By doing this,
-not only do we gain some additional tools that will become handy later down the road, but we also test whether our axioms are behaving as we would like them to.
-**)
+(** Since Coq now understands the basics of Boolean algebra, it serves as a good
+    exercise for us to generate some further rules using Coq's proving systems.
+    By doing this, not only do we gain some additional tools that will become
+    handy later down the road, but we also test whether our axioms are behaving
+    as we would like them to. *)
 
-(* Lemma for a sub-case of term multiplication. *)
+(*  Lemma for a sub-case of term multiplication. *)
 Lemma mul_x_x_plus_T1 :
   forall x, x * (x + T1) == T0.
 Proof.
-intros. rewrite distr. rewrite mul_x_x. rewrite mul_comm. 
-rewrite mul_id. apply sum_x_x.
+  intros. rewrite distr. rewrite mul_x_x. rewrite mul_comm.
+  rewrite mul_id. apply sum_x_x.
 Qed.
 
-(* Lemma to convert term equivalence to equivalence between their
-  addition and ground term T0, and vice-versa. *)
+(*  Lemma to convert term equivalence to equivalence between their
+    addition and ground term T0, and vice-versa. *)
 Lemma x_equal_y_x_plus_y :
   forall x y, x == y <-> x + y == T0.
 Proof.
-intros. split.
-- intros. rewrite H. rewrite sum_x_x. reflexivity.
-- intros. rewrite term_sum_symmetric with (y := y) (z := y). rewrite sum_x_x.
-  apply H.
+  intros. split.
+  - intros. rewrite H. rewrite sum_x_x. reflexivity.
+  - intros. rewrite term_sum_symmetric with (y := y) (z := y). rewrite sum_x_x.
+    apply H.
 Qed.
 
-Hint Resolve mul_x_x_plus_T1.
-Hint Resolve x_equal_y_x_plus_y.
+Hint Resolve mul_x_x_plus_T1 x_equal_y_x_plus_y.
 
-(**
-These lemmas just serve to make certain rewrites regarding the core axioms less tedious to write. While one could certainly argue that they should be formulated as axioms and
-not lemmas due to their triviality, being pedantic is a good exercise.
-**)
+(** These lemmas just serve to make certain rewrites regarding the core axioms
+    less tedious to write. While one could certainly argue that they should be
+    formulated as axioms and not lemmas due to their triviality, being pedantic
+    is a good exercise. *)
 
-(* Lemma for identity addition between term and ground term T0 *)
+(*  Lemma for identity addition between term and ground term T0 *)
 Lemma sum_id_sym :
   forall x, x + T0 == x.
 Proof.
-intros. rewrite sum_comm. apply sum_id.
+  intros. rewrite sum_comm. apply sum_id.
 Qed.
 
-(* Lemma for identity multiplication between term and ground term T1 *)
+(*  Lemma for identity multiplication between term and ground term T1 *)
 Lemma mul_id_sym :
   forall x, x * T1 == x.
 Proof.
-intros. rewrite mul_comm. apply mul_id.
+  intros. rewrite mul_comm. apply mul_id.
 Qed.
 
-(* Lemma for multiplication between term and ground term T0 *)
+(*  Lemma for multiplication between term and ground term T0 *)
 Lemma mul_T0_x_sym :
   forall x, x * T0 == T0.
 Proof.
-intros. rewrite mul_comm. apply mul_T0_x.
+  intros. rewrite mul_comm. apply mul_T0_x.
 Qed.
 
 Lemma sum_assoc_opp :
@@ -235,60 +238,65 @@ Qed.
 
 (** * Variable Sets **)
 
-(**
-Now that the underlying behavior concerning Boolean algebra has been properly articulated to Coq, it is now time to begin
-formalizing the logic surrounding our meta reasoning of Boolean equations and systems. While there are certainly several approaches to begin this process, we thought it best to 
-ease into things through formalizing the notion of a set of variables present in an equation.
-**)
+(** Now that the underlying behavior concerning Boolean algebra has been
+    properly articulated to Coq, it is now time to begin formalizing the logic
+    surrounding our meta reasoning of Boolean equations and systems. While there
+    are certainly several approaches to begin this process, we thought it best
+    to ease into things through formalizing the notion of a set of variables
+    present in an equation. *)
 
 (** ** Definitions **)
 
-(**
-We now define a variable set to be precisely a list of variables; additionally, we include several functions for including and excluding variables from these variable sets. 
-Furthermore, since uniqueness is not a property guaranteed by Coq lists and it has the potential to be desirable, we define a function that consumes a variable set and 
-removes duplicate entries from it. For convenience, we also provide several examples to demonstrate the functionalities of these new definitions.
-**)
+(** We now define a _variable set_ to be precisely a list of variables;
+    additionally, we include several functions for including and excluding
+    variables from these variable sets. Furthermore, since uniqueness is not a
+    property guaranteed by Coq lists and it has the potential to be desirable,
+    we define a function that consumes a variable set and removes duplicate
+    entries from it. For convenience, we also provide several examples to
+    demonstrate the functionalities of these new definitions. *)
 
-(* Definition of new type to represent a list (set) of variables (naturals) *) 
+(*  Definition of new type to represent a list (set) of variables (naturals) *)
 Definition var_set := list var.
 Implicit Type vars: var_set.
 
 
-(* Function to check to see if a variable is in a variable set *)
+(*  Function to check to see if a variable is in a variable set *)
 Fixpoint var_set_includes_var (v : var) (vars : var_set) : bool :=
   match vars with
     | nil => false
-    | n :: n' => if (beq_nat v n) then true else var_set_includes_var v n'
+    | n :: n' => if (beq_nat v n) then true
+                                  else var_set_includes_var v n'
   end.
 
 
-(* Function to remove all instances of v from vars *)
+(*  Function to remove all instances of v from vars *)
 Fixpoint var_set_remove_var (v : var) (vars : var_set) : var_set :=
   match vars with
     | nil => nil
-    | n :: n' => if (beq_nat v n) then (var_set_remove_var v n') else n :: (var_set_remove_var v n')
+    | n :: n' => if (beq_nat v n) then (var_set_remove_var v n')
+                                  else n :: (var_set_remove_var v n')
   end.
 
-(* Function to return a unique var_set without duplicates. Found_vars should be empty for correctness
-   guarantee *)
+(*  Function to return a unique var_set without duplicates. Found_vars should be
+    empty for correctness guarantee *)
 Fixpoint var_set_create_unique (vars : var_set): var_set :=
   match vars with
     | nil => nil
     | n :: n' => 
     if (var_set_includes_var n n') then var_set_create_unique n'
-    else n :: var_set_create_unique n'
+                                   else n :: var_set_create_unique n'
   end.
 
-(* Function to check if a given var_set is unique *)
+(*  Function to check if a given var_set is unique *)
 Fixpoint var_set_is_unique (vars : var_set): bool :=
   match vars with
     | nil => true
     | n :: n' => 
-    if (var_set_includes_var n n') then false 
-    else var_set_is_unique n'
+    if (var_set_includes_var n n') then false
+                                   else var_set_is_unique n'
   end.
 
-(* Function to get the variables of a term as a var_set *)
+(*  Function to get the variables of a term as a var_set *)
 Fixpoint term_vars (t : term) : var_set :=
   match t with
     | T0 => nil
@@ -298,68 +306,66 @@ Fixpoint term_vars (t : term) : var_set :=
     | SUM x y => (term_vars x) ++ (term_vars y)
   end.
 
-(* Function to generate a list of unique variables that make up a given term *)
+(*  Function to generate a list of unique variables that make up a given term *)
 Definition term_unique_vars (t : term) : var_set :=
-  (var_set_create_unique (term_vars t)).
+  var_set_create_unique (term_vars t).
 
 
 Lemma vs_includes_true : forall (x : var) (lvar : list var),
   var_set_includes_var x lvar = true -> In x lvar.
- Proof.
- intros.
+Proof.
+  intros.
   induction lvar.
-  -  simpl; intros.
-  discriminate.
+  - simpl; intros. discriminate.
   - simpl in H. remember (beq_nat x a) as H2. destruct H2.
-  +  simpl. left. symmetry in HeqH2. pose proof beq_nat_true as H7. specialize (H7 x a HeqH2).
-    symmetry in H7.  apply H7.
-  + specialize (IHlvar H). simpl.  right.  apply IHlvar. 
+    + simpl. left. symmetry in HeqH2. pose proof beq_nat_true as H7.
+      specialize (H7 x a HeqH2). symmetry in H7. apply H7.
+    + specialize (IHlvar H). simpl. right. apply IHlvar.
 Qed.
 
 
 Lemma vs_includes_false : forall (x : var) (lvar : list var),
   var_set_includes_var x lvar = false -> ~ In x lvar.
- Proof.
- intros.
+Proof.
+  intros.
   induction lvar.
-  -  simpl; intros. unfold not. intros. destruct H0.
+  - simpl; intros. unfold not. intros. destruct H0.
   - simpl in H. remember (beq_nat x a) as H2. destruct H2. inversion H.
     specialize (IHlvar H). firstorder. intuition. apply IHlvar. simpl in H0.
-    destruct H0. 
-    { inversion HeqH2. symmetry in H2. pose proof beq_nat_false as H7. specialize (H7 x a H2).
-      rewrite H0 in H7. destruct H7. intuition. }
-    {  apply H0. }
+    destruct H0.
+    + inversion HeqH2. symmetry in H2. pose proof beq_nat_false as H7.
+      specialize (H7 x a H2). rewrite H0 in H7. destruct H7. intuition.
+    + apply H0.
 Qed.
 
 
-Lemma in_dup_and_non_dup :
- forall (x: var) (lvar : list var),
- In x lvar <-> In x (var_set_create_unique lvar).
+Lemma in_dup_and_non_dup : forall (x: var) (lvar : list var),
+  In x lvar <-> In x (var_set_create_unique lvar).
 Proof.
- intros. split.
- - induction lvar.
-  +  intros. simpl in H. destruct H.
-  + intros. simpl. remember(var_set_includes_var a lvar) as C. destruct C.
-   { symmetry in HeqC. pose proof vs_includes_true as H7. specialize (H7 a lvar HeqC).
-     simpl in H. destruct H. 
-    { rewrite H in H7. specialize (IHlvar H7). apply IHlvar. }
-    { specialize (IHlvar H). apply IHlvar. }
-   }
-   { symmetry in HeqC. pose proof vs_includes_false as H7. specialize (H7 a lvar HeqC).
-     simpl in H. destruct H.
-    { simpl.  left.  apply H. }
-    {  specialize (IHlvar H). simpl. right. apply IHlvar. }
-   } 
- - induction lvar.
-   + intros.  simpl in H. destruct H.
-   +  intros. simpl in H. remember(var_set_includes_var a lvar) as C. destruct C.
-     { symmetry in HeqC. pose proof vs_includes_true as H7. specialize (H7 a lvar HeqC).
-      specialize (IHlvar H). simpl.  right. apply IHlvar. }
-     { symmetry in HeqC. pose proof vs_includes_false as H7. specialize (H7 a lvar HeqC).
-       simpl in H. destruct H.
-      { simpl.  left. apply H. }
-      { specialize (IHlvar H).  simpl. right. apply IHlvar. } }
-Qed.  
+  intros. split.
+  - induction lvar.
+    + intros. simpl in H. destruct H.
+    + intros. simpl. remember (var_set_includes_var a lvar) as C. destruct C.
+      * symmetry in HeqC. pose proof vs_includes_true as H7.
+        specialize (H7 a lvar HeqC). simpl in H. destruct H.
+        -- rewrite H in H7. specialize (IHlvar H7). apply IHlvar.
+        -- specialize (IHlvar H). apply IHlvar.
+      * symmetry in HeqC. pose proof vs_includes_false as H7.
+        specialize (H7 a lvar HeqC). simpl in H. destruct H.
+        -- simpl. left. apply H.
+        -- specialize (IHlvar H). simpl. right. apply IHlvar.
+  - induction lvar.
+    + intros. simpl in H. destruct H.
+    + intros. simpl in H. remember (var_set_includes_var a lvar) as C.
+      destruct C.
+      * symmetry in HeqC. pose proof vs_includes_true as H7.
+        specialize (H7 a lvar HeqC). specialize (IHlvar H). simpl.
+        right. apply IHlvar.
+      * symmetry in HeqC. pose proof vs_includes_false as H7.
+        specialize (H7 a lvar HeqC). simpl in H. destruct H.
+        -- simpl.  left. apply H.
+        -- specialize (IHlvar H).  simpl. right. apply IHlvar.
+Qed.
 
 
 (** ** Examples **)
@@ -367,352 +373,308 @@ Qed.
 Example var_set_create_unique_ex1 :
   var_set_create_unique [0;5;2;1;1;2;2;9;5;3] = [0;1;2;9;5;3].
 Proof.
-simpl. reflexivity.
+  simpl. reflexivity.
 Qed.
 
 Example var_set_is_unique_ex1 :
   var_set_is_unique [0;2;2;2] = false.
 Proof.
-simpl. reflexivity.
+  simpl. reflexivity.
 Qed.
 
-(* Examples to prove the correctness of the function term_vars on specific cases *)
+(*  Examples to prove the correctness of the function term_vars on specific
+    cases *)
 
 Example term_vars_ex1 :
   term_vars (VAR 0 + VAR 0 + VAR 1) = [0;0;1].
 Proof.
-simpl. reflexivity.
+  simpl. reflexivity.
 Qed.
 
 Example term_vars_ex2 :
   In 0 (term_vars (VAR 0 + VAR 0 + VAR 1)).
 Proof.
-simpl. left. reflexivity.
+  simpl. left. reflexivity.
 Qed.
 
 (** * Ground Terms **)
 
-(**
-Seeing as we just outlined the definition of a variable set, it seems fair to now formalize the definition of a ground term, or in other words, a term that has no variables and whose 
-variable set is the empty set.
-**)
+(** Seeing as we just outlined the definition of a variable set, it seems fair
+    to now formalize the definition of a ground term, or in other words, a term
+    that has no variables and whose variable set is the empty set. *)
 
 (** ** Definitions **)
 
-(** 
-A ground term is a recursively defined proposition that is only True if and only if no variable appears in it; otherwise it will be a False proposition and no longer
-a ground term.
-**)
+(** A _ground term_ is a recursively defined proposition that is only true if
+    and only if no variable appears in it; otherwise it will be a false
+    proposition and no longer a ground term. *)
 
-(* In this subsection we declare definitions related to ground terms, inluding 
-  functions and lemmas *)
+(*  In this subsection we declare definitions related to ground terms, inluding
+    functions and lemmas *)
 
-(* Function to check if a given term is a ground term (i.e. has no vars)*)
+(*  Function to check if a given term is a ground term (i.e. has no vars) *)
 Fixpoint ground_term (t : term) : Prop :=
   match t with
     | VAR x => False
-    | SUM x y => (ground_term x) /\ (ground_term y)
-    | PRODUCT x y => (ground_term x) /\ (ground_term y)
+    | SUM x y => ground_term x /\ ground_term y
+    | PRODUCT x y => ground_term x /\ ground_term y
     | _ => True
   end.
 
 (** ** Lemmas **)
 
-(**
-Our first real lemma (shown below), articulates an important property of ground terms: all ground terms are equvialent to either 0 or 1. This curious property is a 
-direct result of the fact that these terms possess no variables and additioanlly because of the axioms of Boolean algebra.
-**)
+(** Our first real lemma (shown below), articulates an important property of
+    ground terms: all ground terms are equvialent to either [0] or [1]. This
+    curious property is a direct result of the fact that these terms possess no
+    variables and additioanlly because of the axioms of Boolean algebra. *)
 
-(* Lemma (trivial, intuitively true) that proves that if the function ground_term returns
-   true then it is either T0 or T1 *) 
+(*  Lemma (trivial, intuitively true) that proves that if the function
+    ground_term returns true then it is either T0 or T1 *)
 Lemma ground_term_equiv_T0_T1 :
-  forall x, (ground_term x) -> (x == T0 \/ x == T1).
+  forall x, ground_term x -> x == T0 \/ x == T1.
 Proof.
-intros. induction x.
-- left. reflexivity.
-- right. reflexivity.
-- contradiction.
-- inversion H. destruct IHx1; destruct IHx2; auto. rewrite H2. left. rewrite sum_id. 
-apply H3. 
-rewrite H2. rewrite H3. rewrite sum_id. right. reflexivity.
-rewrite H2. rewrite H3. right. rewrite sum_comm. rewrite sum_id. reflexivity.
-rewrite H2. rewrite H3. rewrite sum_x_x. left. reflexivity.
-- inversion H. destruct IHx1; destruct IHx2; auto. rewrite H2. left. rewrite mul_T0_x. reflexivity.
-rewrite H2. left. rewrite mul_T0_x. reflexivity.
-rewrite H3. left. rewrite mul_comm. rewrite mul_T0_x. reflexivity. 
-rewrite H2. rewrite H3. right. rewrite mul_id. reflexivity. 
+  intros. induction x.
+  - left. reflexivity.
+  - right. reflexivity.
+  - contradiction.
+  - inversion H. destruct IHx1; destruct IHx2; auto. rewrite H2. left.
+    rewrite sum_id. apply H3. rewrite H2. rewrite H3. rewrite sum_id. right.
+    reflexivity. rewrite H2. rewrite H3. right. rewrite sum_comm.
+    rewrite sum_id. reflexivity. rewrite H2. rewrite H3. rewrite sum_x_x. left.
+    reflexivity.
+  - inversion H. destruct IHx1; destruct IHx2; auto. rewrite H2. left.
+    rewrite mul_T0_x. reflexivity. rewrite H2. left. rewrite mul_T0_x.
+    reflexivity. rewrite H3. left. rewrite mul_comm. rewrite mul_T0_x.
+    reflexivity. rewrite H2. rewrite H3. right. rewrite mul_id. reflexivity.
 Qed.
 
-(** 
-This lemma, while intuitively obvious by definition, nonetheless provides a formal bridge between the world of ground terms and the world of variable sets.
-**)
+(** This lemma, while intuitively obvious by definition, nonetheless provides a
+    formal bridge between the world of ground terms and the world of variable
+    sets. *)
 
 Lemma ground_term_has_empty_var_set :
   forall x, (ground_term x) -> (term_vars x) = [].
 Proof.
-intros. induction x.
-- simpl. reflexivity.
-- simpl. reflexivity.
-- contradiction.
-- firstorder. unfold term_vars. unfold term_vars in H2. rewrite H2. unfold term_vars in H1. rewrite H1. simpl. reflexivity.
-- firstorder. unfold term_vars. unfold term_vars in H2. rewrite H2. unfold term_vars in H1. rewrite H1. simpl. reflexivity.
+  intros. induction x.
+  - simpl. reflexivity.
+  - simpl. reflexivity.
+  - contradiction.
+  - firstorder. unfold term_vars. unfold term_vars in H2. rewrite H2.
+    unfold term_vars in H1. rewrite H1. simpl. reflexivity.
+  - firstorder. unfold term_vars. unfold term_vars in H2. rewrite H2.
+    unfold term_vars in H1. rewrite H1. simpl. reflexivity.
 Qed.
 
 (** ** Examples **)
 
-(** Here are some examples to show that our ground term definition is working appropriately. **)
+(** Here are some examples to show that our ground term definition is working
+    appropriately. *)
 
 Example ex_gt1 :
-  (ground_term (T0 + T1)).
+  ground_term (T0 + T1).
 Proof.
-simpl. split. 
-- reflexivity.
-- reflexivity.
+  simpl. split.
+  - reflexivity.
+  - reflexivity.
 Qed.
 
 Example ex_gt2 :
-  (ground_term (VAR 0 * T1)) -> False.
+  ground_term (VAR 0 * T1) -> False.
 Proof.
-simpl. intros. destruct H. apply H.
+  simpl. intros. destruct H. apply H.
 Qed.
 
 (** * Substitutions **)
 
-(** 
-It is at this point in our Coq development that we begin to officially define the principal action around which the entirety of our efforts are
-centered: the act of substituting variables with other terms. While substitutions alone are not of great interest, their emergent properties
-as in the case of whether or not a given substitution unifies an equation are of substantial importance to our later research.
-**)
+(** It is at this point in our Coq development that we begin to officially
+    define the principal action around which the entirety of our efforts are
+    centered: the act of substituting variables with other terms. While
+    substitutions alone are not of great interest, their emergent properties as
+    in the case of whether or not a given substitution unifies an equation are
+    of substantial importance to our later research. *)
 
 (** ** Definitions **)
 
-(* In this sub-section we make the fundamental definitions of substitutions, basic functions
- for them, accompanying lemmas and some propsitions *)
+(** In this subsection we make the fundamental definitions of substitutions,
+    basic functions for them, accompanying lemmas and some propsitions. *)
 
-(**
-Here we define a substitution to be a list of ordered pairs where each pair represents a variable being mapped to a term. For sake of clarity
-these ordered pairs shall be referred to as replacements from now on and as a result, substitutions should really be considered to be lists
-of replacements.
-**)
+(** Here we define a _substitution_ to be a list of ordered pairs where each
+    pair represents a variable being mapped to a term. For sake of clarity these
+    ordered pairs shall be referred to as _replacements_ from now on and as a
+    result, substitutions should really be considered to be lists of
+    replacements. *)
 
-Definition replacement := (prod var term).
+Definition replacement := prod var term.
 
-(* We define a new type susbt to represent a substitution as a list of replacements *)
+(*  We define a new type susbt to represent a substitution as a list of
+    replacements *)
 Definition subst := list replacement.
 
 Implicit Type s : subst.
 
-(** 
-Our first function, find_replacement, is an auxilliary to apply_subst. This function will search through a substitution for a specific
-variable, and if found, returns the variable's associated term.
-**)
+(** Our first function, [find_replacement], is an auxilliary to [apply_subst].
+    This function will search through a substitution for a specific variable,
+    and if found, returns the variable's associated term. *)
 
 Fixpoint find_replacement (x : var) (s : subst) : term :=
-  match s with 
+  match s with
   | nil => VAR x
   | r :: r' =>
-      if beq_nat (fst r) x then (snd r)
-      else
-        (find_replacement x r')
+      if beq_nat (fst r) x then snd r
+                           else find_replacement x r'
   end.
 
-(**
-The apply_subst function will take a term and a substitution and will produce a new term reflecting the changes made to the original one.
-**)
+(** The [apply_subst] function will take a term and a substitution and will
+    produce a new term reflecting the changes made to the original one. *)
 
 Fixpoint apply_subst (t : term) (s : subst) : term :=
-  match t with 
+  match t with
   | T0 => T0
-  | T1 => T1 
-  | VAR x => (find_replacement x s)
+  | T1 => T1
+  | VAR x => find_replacement x s
   | PRODUCT x y => PRODUCT (apply_subst x s) (apply_subst y s)
   | SUM x y => SUM (apply_subst x s) (apply_subst y s)
   end.
 
-(**
-For reasons of completeness, it is useful to be able to generate identity substitutions; namely, substitutions that map the variables of a 
-term's variable set to themselves.
-**)
+(** For reasons of completeness, it is useful to be able to generate _identity
+    substitutions_; namely, substitutions that map the variables of a term to
+    themselves. *)
 
-(* function that given a list of variables, it build a list of identical substitutions - one for each variable *)
+(*  function that given a list of variables, it build a list of identical
+    substitutions - one for each variable *)
 Fixpoint build_id_subst (lvar : var_set) : subst :=
   match lvar with
   | nil => nil
-  | v :: v' => (cons (v , (VAR v))  
-                      (build_id_subst v'))
+  | v :: v' => (v , (VAR v)) :: build_id_subst v'
   end.
 
-(**
-Since we now have the ability to generate identity substitutions, we should now formalize a general proposition for testing whether or not a 
-given substitution is an identity substitution of a given term.
-**)
+(** Since we now have the ability to generate identity substitutions, we should
+    now formalize a general proposition for testing whether or not a given
+    substitution is an identity substitution of a given term. *)
 
 Definition subst_equiv (s1 s2: subst) : Prop :=
   forall t, apply_subst t s1 == apply_subst t s2.
 
 Definition subst_is_id_subst (t : term) (s : subst) : Prop :=
-  (apply_subst t s) == t.
+  apply_subst t s == t.
 
 (** ** Lemmas **)
 
-(**
-Having now outlined the functionality of a subsitution, let us now begin to analyze some implications of its form and composition by proving some
-lemmas.
-**)
+(** Having now outlined the functionality of a subsitution, let us now begin to
+    analyze some implications of its form and composition by proving some
+    lemmas. *)
 
-(**
-Given that we have a definition for identity substitutions, we should prove that identity substitutions do not modify
-a term.
-**)
+(** Given that we have a definition for identity substitutions, we should prove
+    that identity substitutions do not modify a term. *)
 
-Lemma id_subst:
-  forall (t : term) (l : var_set),
+Lemma id_subst: forall (t : term) (l : var_set),
   apply_subst t (build_id_subst l) == t.
 Proof.
-intros. induction t.
-{
-  simpl. reflexivity.
-}
-{
-  simpl. reflexivity.
-}
-{
-  simpl. induction l.
-  {
-    simpl. reflexivity.
-  }
-  {
-    simpl. destruct (beq_nat a v) eqn: e.
-    {
-      apply beq_nat_true in e. rewrite e. reflexivity.
-    }
-    {
-      apply IHl.
-    }
-  }
-}
-{
-  simpl. rewrite IHt1. rewrite IHt2. reflexivity.
-}
-{
-  simpl. rewrite IHt1. rewrite IHt2. reflexivity.
-}
+  intros. induction t.
+  - simpl. reflexivity.
+  - simpl. reflexivity.
+  - simpl. induction l.
+    + simpl. reflexivity.
+    + simpl. destruct (beq_nat a v) eqn: e.
+      * apply beq_nat_true in e. rewrite e. reflexivity.
+      * apply IHl.
+  - simpl. rewrite IHt1. rewrite IHt2. reflexivity.
+  - simpl. rewrite IHt1. rewrite IHt2. reflexivity.
 Qed.
 
-(* Helper lemmeas for proving apply_subst_compat *)
+(*  Helper lemmeas for proving apply_subst_compat *)
 
-Lemma sum_comm_compat t1 t2:
-  forall (sigma: subst), (apply_subst (t1 + t2) sigma) == (apply_subst (t2 + t1) sigma).
+Lemma sum_comm_compat t1 t2: forall (sigma: subst),
+  apply_subst (t1 + t2) sigma == apply_subst (t2 + t1) sigma.
 Proof.
-  intros.
-  simpl.
-  auto.
+  intros. simpl. auto.
 Qed.
 Hint Resolve sum_comm_compat.
 
-Lemma sum_assoc_compat t1 t2 t3:
-  forall (sigma: subst), (apply_subst ((t1 + t2) + t3) sigma) == (apply_subst (t1 + (t2 + t3)) sigma).
+Lemma sum_assoc_compat t1 t2 t3: forall (sigma: subst),
+  apply_subst ((t1 + t2) + t3) sigma == apply_subst (t1 + (t2 + t3)) sigma.
 Proof.
-  intros.
-  simpl.
-  auto.
+  intros. simpl. auto.
 Qed.
 Hint Resolve sum_assoc_compat.
 
-Lemma sum_id_compat t:
-  forall (sigma: subst), (apply_subst (T0 + t) sigma) == (apply_subst t sigma).
+Lemma sum_id_compat t: forall (sigma: subst),
+  apply_subst (T0 + t) sigma == apply_subst t sigma.
 Proof.
-  intros.
-  simpl.
-  auto.
+  intros. simpl. auto.
 Qed.
 Hint Resolve sum_id_compat.
 
-Lemma sum_x_x_compat t:
-  forall (sigma: subst), (apply_subst (t + t) sigma) == (apply_subst T0 sigma).
+Lemma sum_x_x_compat t: forall (sigma: subst),
+  apply_subst (t + t) sigma == apply_subst T0 sigma.
 Proof.
-  intros.
-  simpl.
-  auto.
+  intros. simpl. auto.
 Qed.
 Hint Resolve sum_x_x_compat.
 
-Lemma mul_comm_compat t1 t2:
-  forall (sigma: subst), (apply_subst (t1 * t2) sigma) == (apply_subst (t2 * t1) sigma).
+Lemma mul_comm_compat t1 t2: forall (sigma: subst),
+  apply_subst (t1 * t2) sigma == apply_subst (t2 * t1) sigma.
 Proof.
-  intros.
-  simpl.
-  auto.
+  intros. simpl. auto.
 Qed.
 Hint Resolve mul_comm_compat.
 
-Lemma mul_assoc_compat t1 t2 t3:
-  forall (sigma: subst), (apply_subst ((t1 * t2) * t3) sigma) == (apply_subst (t1 * (t2 * t3)) sigma).
+Lemma mul_assoc_compat t1 t2 t3: forall (sigma: subst),
+  apply_subst ((t1 * t2) * t3) sigma == apply_subst (t1 * (t2 * t3)) sigma.
 Proof.
-  intros.
-  simpl.
-  auto.
+  intros. simpl. auto.
 Qed.
 Hint Resolve mul_assoc_compat.
 
-Lemma mul_x_x_compat t:
-  forall (sigma: subst), (apply_subst (t * t) sigma) == (apply_subst t sigma).
+Lemma mul_x_x_compat t: forall (sigma: subst),
+  apply_subst (t * t) sigma == apply_subst t sigma.
 Proof.
-  intros sigma.
-  simpl.
-  auto.
+  intros. simpl. auto.
 Qed.
 Hint Resolve mul_x_x_compat.
 
-Lemma mul_T0_x_compat t:
-  forall (sigma: subst), (apply_subst (T0 * t) sigma) == (apply_subst T0 sigma).
+Lemma mul_T0_x_compat t: forall (sigma: subst),
+  apply_subst (T0 * t) sigma == apply_subst T0 sigma.
 Proof.
-  intros.
-  simpl.
-  auto.
+  intros. simpl. auto.
 Qed.
 Hint Resolve mul_T0_x_compat.
 
-Lemma mul_id_compat t:
-  forall (sigma: subst), (apply_subst (T1 * t) sigma) == (apply_subst t sigma).
+Lemma mul_id_compat t: forall (sigma: subst),
+  apply_subst (T1 * t) sigma == apply_subst t sigma.
 Proof.
-  intros.
-  simpl.
-  auto.
+  intros. simpl. auto.
 Qed.
 Hint Resolve mul_id_compat.
 
-Lemma distr_compat t1 t2 t3:
-  forall (sigma: subst), (apply_subst (t1 * (t2 + t3)) sigma) == (apply_subst ((t1 * t2) + (t1 * t3)) sigma).
+Lemma distr_compat t1 t2 t3: forall (sigma: subst),
+  apply_subst (t1 * (t2 + t3)) sigma ==
+  apply_subst ((t1 * t2) + (t1 * t3)) sigma.
 Proof.
-  intros.
-  simpl.
-  auto.
+  intros. simpl. auto.
 Qed.
 Hint Resolve distr_compat.
 
-Lemma refl_comm_compat t1 t2:
-  forall (sigma: subst), (apply_subst t1 sigma) == (apply_subst t2 sigma) -> (apply_subst t2 sigma) == (apply_subst t1 sigma).
+Lemma refl_comm_compat t1 t2: forall (sigma: subst),
+  apply_subst t1 sigma == apply_subst t2 sigma ->
+  apply_subst t2 sigma == apply_subst t1 sigma.
 Proof.
-  intros.
-  simpl.
-  auto.
+  intros. simpl. auto.
 Qed.
 Hint Resolve refl_comm_compat.
 
-Lemma trans_compat t1 t2 t3 :
-  forall (sigma: subst),
-    (apply_subst t1 sigma) == (apply_subst t2 sigma) ->
-    (apply_subst t2 sigma) == (apply_subst t3 sigma) ->
-    (apply_subst t1 sigma) == (apply_subst t3 sigma) .
+Lemma trans_compat t1 t2 t3 : forall (sigma: subst),
+  apply_subst t1 sigma == apply_subst t2 sigma ->
+  apply_subst t2 sigma == apply_subst t3 sigma ->
+  apply_subst t1 sigma == apply_subst t3 sigma.
 Proof.
-  intros sigma H12 H23.
-  eauto.
+  intros. eauto.
 Qed.
 Hint Resolve trans_compat.
 
-Lemma apply_subst_compat : forall  (t t' : term),
-     t == t' -> forall (sigma: subst), (apply_subst t sigma) == (apply_subst t' sigma).
+Lemma apply_subst_compat : forall (t t' : term),
+  t == t' ->
+  forall (sigma: subst), apply_subst t sigma == apply_subst t' sigma.
 Proof.
 Admitted.
 
@@ -722,484 +684,475 @@ Proof.
   exact apply_subst_compat.
 Qed.
 
-(**
-An easy thing to prove right off the bat is that ground terms, i.e. terms with no variables, cannot be modified by applying substitutions to 
-them. This will later prove to be very relevant when we begin to talk about unification.
-**)
+(** An easy thing to prove right off the bat is that ground terms, i.e. terms
+    with no variables, cannot be modified by applying substitutions to them.
+    This will later prove to be very relevant when we begin to talk about
+    unification. *)
 
-(* Helpful lemma for showing substitutions do not affect ground terms *)
-Lemma ground_term_cannot_subst :
-  forall x, (ground_term x) -> (forall s, apply_subst x s == x).
+(*  Helpful lemma for showing substitutions do not affect ground terms *)
+Lemma ground_term_cannot_subst : forall x,
+  ground_term x ->
+  forall s, apply_subst x s == x.
 Proof.
-intros. induction s. 
+  intros. induction s.
   - apply ground_term_equiv_T0_T1 in H. destruct H.
-  + rewrite H. simpl. reflexivity.
-  + rewrite H. simpl. reflexivity.
+    + rewrite H. simpl. reflexivity.
+    + rewrite H. simpl. reflexivity.
   - apply ground_term_equiv_T0_T1 in H. destruct H. rewrite H.
-    +  simpl. reflexivity.
+    + simpl. reflexivity.
     + rewrite H. simpl. reflexivity.
 Qed.
 
-(**
-A fundamental property of substitutions is their distributivity and associativity across the summation and multiplication of terms.
-Again the importance of these proofs will not become apparent until we talk about unification.
-**)
+(** A fundamental property of substitutions is their distributivity and
+    associativity across the summation and multiplication of terms. Again the
+    importance of these proofs will not become apparent until we talk about
+    unification. *)
 
-(* A useful lemma for showing the distributivity of substitutions across terms *)
-Lemma subst_distribution :
-  forall s x y, apply_subst x s + apply_subst y s == apply_subst (x + y) s.
+(*  A useful lemma for showing the distributivity of substitutions across terms
+    *)
+Lemma subst_distribution : forall s x y,
+  apply_subst x s + apply_subst y s == apply_subst (x + y) s.
 Proof.
-intro. induction s. simpl. intros. reflexivity. intros. simpl. reflexivity. 
+  intro. induction s.
+  - simpl. intros. reflexivity.
+  - intros. simpl. reflexivity.
 Qed.
 
-(* A lemma to prove the associativity of the apply_subst function *)
-Lemma subst_associative :
-  forall s x y, apply_subst x s * apply_subst y s == apply_subst (x * y) s.
+(*  A lemma to prove the associativity of the apply_subst function *)
+Lemma subst_associative : forall s x y,
+  apply_subst x s * apply_subst y s == apply_subst (x * y) s.
 Proof.
-intro. induction s. intros. reflexivity. intros. simpl. reflexivity. 
+  intro. induction s.
+  - intros. reflexivity.
+  - intros. simpl. reflexivity. 
 Qed.
 
-
-Lemma subst_sum_distr_opp :
-  forall s x y, apply_subst (x + y) s == apply_subst x s + apply_subst y s.
+Lemma subst_sum_distr_opp : forall s x y,
+  apply_subst (x + y) s == apply_subst x s + apply_subst y s.
 Proof.
   intros.
   apply refl_comm.
   apply subst_distribution.
-Qed. 
+Qed.
 
-
-Lemma subst_mul_distr_opp :
-  forall s x y, apply_subst (x * y) s == apply_subst x s * apply_subst y s.
+Lemma subst_mul_distr_opp : forall s x y,
+  apply_subst (x * y) s == apply_subst x s * apply_subst y s.
 Proof.
   intros.
   apply refl_comm.
   apply subst_associative.
-Qed. 
+Qed.
 
-Lemma var_subst:
-  forall (v : var) (ts : term) ,
-  (apply_subst (VAR v) (cons (v , ts) nil) ) == ts.
+Lemma var_subst: forall (v : var) (ts : term),
+  apply_subst (VAR v) [(v , ts)] == ts.
 Proof.
-intros. simpl. destruct (beq_nat v v) eqn: e. apply beq_nat_true in e.
-reflexivity. apply beq_nat_false in e. firstorder.
+  intros. simpl. destruct (beq_nat v v) eqn: e.
+  - apply beq_nat_true in e. reflexivity.
+  - apply beq_nat_false in e. firstorder.
 Qed.
 
 (** ** Examples **)
 
-(**
-Here are some examples showcasing the nature of applying substitutions to terms.
-**)
+(** Here are some examples showcasing the nature of applying substitutions to
+    terms. *)
 
 Example subst_ex1 :
-  (apply_subst (T0 + T1) []) == T0 + T1.
+  apply_subst (T0 + T1) [] == T0 + T1.
 Proof.
-intros. reflexivity.
+  intros. reflexivity.
 Qed.
 
 Example subst_ex2 :
-  (apply_subst (VAR 0 * VAR 1) [(0, T0)]) == T0.
+  apply_subst (VAR 0 * VAR 1) [(0, T0)] == T0.
 Proof.
-intros. simpl. apply mul_T0_x.
+  intros. simpl. apply mul_T0_x.
 Qed.
 
 (** * Unification **)
 
-(**
-Now that we have established the concept of term substitutions in Coq, it is time for us to formally define the concept of 
-Boolean unification. Unification, in its most literal sense, refers to the act of applying a substitution to terms in order
-to make them equivalent to each other. In other words, to say that two terms are unifiable is to really say that there exists
-a substitution such that the two terms are equal. Interestingly enough, we can abstract this concept further to simply saying
-that a single term is unifiable if there exists a substitution such that the term will be equivalent to 0. By doing this 
-abstraction, we can prove that equation solving and unification are essentially the same fundamental problem.
-**)
+(** Now that we have established the concept of term substitutions in Coq, it is
+    time for us to formally define the concept of Boolean unification.
+    _Unification_, in its most literal sense, refers to the act of applying a
+    substitution to terms in order to make them equivalent to each other. In
+    other words, to say that two terms are _unifiable_ is to really say that
+    there exists a substitution such that the two terms are equal. Interestingly
+    enough, we can abstract this concept further to simply saying that a single
+    term is unifiable if there exists a substitution such that the term will be
+    equivalent to [0]. By doing this abstraction, we can prove that equation
+    solving and unification are essentially the same fundamental problem. *)
 
-(**
-Below is the initial definition for unification, namely that two terms can be unified to be equivalent to one another. By starting
-here we will show each step towards abstracting unification to refer to a single term.
-**)
+(** Below is the initial definition for unification, namely that two terms can
+    be unified to be equivalent to one another. By starting here we will show
+    each step towards abstracting unification to refer to a single term. *)
 
-(*
-Definition subst_idempotent (s : subst) : Prop :=
-  forall t, apply_subst t s == apply_subst (apply_subst t s) s.
-*)
-(* Proposition that a given substitution unifies (namely, makes equivalent), two
-  given terms *)
+(*  Proposition that a given substitution unifies (namely, makes equivalent),
+    two given terms *)
 Definition unifies (a b : term) (s : subst) : Prop :=
-  (apply_subst a s) == (apply_subst b s).
+  apply_subst a s == apply_subst b s.
 
-(**
-Here is a simple example demonstrating the concept of testing whether two terms are unified by a substitution.
-**)
+(** Here is a simple example demonstrating the concept of testing whether two
+    terms are unified by a substitution. *)
 
-(* Examples that prove the correctness of the unifies definition *)
+(*  Examples that prove the correctness of the unifies definition *)
 
 Example ex_unif1 :
-  unifies (VAR 0) (VAR 1) ((0, T1) :: (1, T1) :: nil).
+  unifies (VAR 0) (VAR 1) [(0, T1); (1, T1)].
 Proof.
-unfold unifies. simpl. reflexivity.
+  unfold unifies. simpl. reflexivity.
 Qed.
 
-(**
-Now we are going to show that moving both terms to one side of the equivalence relation through addition does not change the 
-concept of unification.
-**)
+(** Now we are going to show that moving both terms to one side of the
+    equivalence relation through addition does not change the concept of
+    unification. *)
 
-(* Proposition that a given substitution makes equivalent the sum of two terms when the substitution 
-  is applied to each of them, and ground term T0 *) 
+(*  Proposition that a given substitution makes equivalent the sum of two terms
+    when the substitution is applied to each of them, and ground term T0 *)
 Definition unifies_T0 (a b : term) (s : subst) : Prop :=
-  (apply_subst a s) + (apply_subst b s) == T0.
+  apply_subst a s + apply_subst b s == T0.
 
-(* Lemma that proves that finding a unifier for x = y is the same as finding a unifier for x + y = 0 *)
-Lemma unifies_T0_equiv :
-  forall x y s, unifies x y s <-> unifies_T0 x y s.
+(*  Lemma that proves that finding a unifier for x = y is the same as finding a
+    unifier for x + y = 0 *)
+Lemma unifies_T0_equiv : forall x y s,
+  unifies x y s <-> unifies_T0 x y s.
 Proof.
-intros. split.
-{ 
-  intros. unfold unifies_T0. unfold unifies in H. rewrite H.
-  rewrite sum_x_x. reflexivity.
-}
-{ 
-  intros. unfold unifies_T0 in H. unfold unifies. 
-  rewrite term_sum_symmetric with (x := apply_subst x s + apply_subst y s) 
-  (z := apply_subst y s) in H. rewrite sum_id in H.
-  rewrite sum_comm in H.
-  rewrite sum_comm with (y := apply_subst y s) in H.
-  rewrite <- sum_assoc in H.
-  rewrite sum_x_x in H.
-  rewrite sum_id in H.
-  apply H.
-}
+  intros. split.
+  - intros. unfold unifies_T0. unfold unifies in H. rewrite H.
+    rewrite sum_x_x. reflexivity.
+  - intros. unfold unifies_T0 in H. unfold unifies.
+    rewrite term_sum_symmetric with (x := apply_subst x s + apply_subst y s) 
+    (z := apply_subst y s) in H. rewrite sum_id in H.
+    rewrite sum_comm in H.
+    rewrite sum_comm with (y := apply_subst y s) in H.
+    rewrite <- sum_assoc in H.
+    rewrite sum_x_x in H.
+    rewrite sum_id in H.
+    apply H.
 Qed.
 
-(**
-Now we can define what it means for a substitution to be a unifier for a given term.
-**)
+(** Now we can define what it means for a substitution to be a unifier for a
+    given term. *)
 
-(* Is 's' a unifier for t? *)
-(* Proposition that a given substitution unifies a given term, namely it makes it
- equivalent with T0. *)
+(*  Is 's' a unifier for t? *)
+(*  Proposition that a given substitution unifies a given term, namely it makes
+    it equivalent with T0. *)
 Definition unifier (t : term) (s : subst) : Prop :=
-  (apply_subst t s) == T0.
+  apply_subst t s == T0.
 
-Example unifier_ex1 : 
-  (unifier (VAR 0) ((0, T0) :: nil)).
+Example unifier_ex1 :
+  unifier (VAR 0) [(0, T0)].
 Proof.
-unfold unifier. simpl. reflexivity.
+  unfold unifier. simpl. reflexivity.
 Qed.
 
-(**
-To ensure our efforts were not in vain, let us now prove that this last abstraction of the unification problem is still 
-equivalent to the original.
-**)
+(** To ensure our efforts were not in vain, let us now prove that this last
+    abstraction of the unification problem is still equivalent to the original.
+    *)
 
-(* Lemma that proves that the unifier proposition can distributes over addition of terms *) 
-Lemma unifier_distribution : 
-  forall x y s, (unifies_T0 x y s) <-> (unifier (x + y) s).
+(*  Lemma that proves that the unifier proposition can distributes over addition
+    of terms *)
+Lemma unifier_distribution : forall x y s,
+  unifies_T0 x y s <-> unifier (x + y) s.
 Proof.
-intros. split.
-{ 
-  intros. unfold unifies_T0 in H. unfold unifier.
-  rewrite <- H. symmetry. apply subst_distribution.
-}
-{ 
-  intros. unfold unifies_T0. unfold unifier in H.
-  rewrite <- H. apply subst_distribution. 
-}
+  intros. split.
+  - intros. unfold unifies_T0 in H. unfold unifier.
+    rewrite <- H. symmetry. apply subst_distribution.
+  - intros. unfold unifies_T0. unfold unifier in H.
+    rewrite <- H. apply subst_distribution.
 Qed.
 
 
-(**
-Lastly let us define a term to be unifiable if there exists a substitution that unifies it.
-**)
+(** Lastly let us define a term to be unifiable if there exists a substitution
+    that unifies it. *)
 
-(* Proposition that states when a term is unifiable *)
+(*  Proposition that states when a term is unifiable *)
 Definition unifiable (t : term) : Prop :=
   exists s, unifier t s.
 
 Example unifiable_ex1 :
   exists x, unifiable (x + T1).
 Proof.
-exists (T1). unfold unifiable. unfold unifier. 
-exists nil. simpl. rewrite sum_x_x. reflexivity.
+  exists T1. unfold unifiable. unfold unifier.
+  exists []. simpl. rewrite sum_x_x. reflexivity.
 Qed.
 
 (** * Most General Unifier **)
 
-(* In this subsection we define propositions, lemmas and examples related 
-  to the most general unifier *)
+(** In this subsection we define propositions, lemmas and examples related to
+    the most general unifier. *)
 
-(**
-  While the property of a term being unifiable is certainly important, it should come as no surprise that not all
-unifiers are created equal; in fact, certain unifiers possess the desirable property of being more general than others. 
-For this reason, let us now formally define the concept of a most general unifier (mgu): a unifier such that with respect to
-a given term, all other unifiers are instances of it, or in other words, less general than it. 
-**)
+(** While the property of a term being unifiable is certainly important, it
+    should come as no surprise that not all unifiers are created equal; in fact,
+    certain unifiers possess the desirable property of being _more general_ than
+    others. For this reason, let us now formally define the concept of a _most
+    general unifier_ (mgu): a unifier such that with respect to a given term,
+    all other unifiers are instances of it, or in other words, less general than
+    it. *)
 
-(**
-  The first step towards establishing the concept of a mgu requires us to formalize
-the notion of a unifier being more general than another. To accomplish this goal, let us formulate the definition
-of a substitution composing another one; or in other words, to say that a substitution is more general than
-another one.
-**)
+(** The first step towards establishing the concept of a mgu requires us to
+    formalize the notion of a unifier being more general than another. To
+    accomplish this goal, let us formulate the definition of a substitution
+    composing another one; or in other words, to say that a substitution is more
+    general than another one. *)
 
-(* substitution composition *)
+(*  substitution composition *)
 Definition substitution_composition (s s' delta : subst) (t : term) : Prop :=
-  forall (x : var), apply_subst (apply_subst (VAR x) s) delta == apply_subst (VAR x) s' .
+  forall (x : var), apply_subst (apply_subst (VAR x) s) delta ==
+                    apply_subst (VAR x) s' .
 
-(* more general unifier *)
+(*  more general unifier *)
 Definition more_general_substitution (s s': subst) (t : term) : Prop :=
   exists delta, substitution_composition s s' delta t.
 
-(**
-  Now that we have articulated the concept of composing substitutions, let us now formulate
-the definition for a most general unifier.
-**)
+(** Now that we have articulated the concept of composing substitutions, let us
+    now formulate the definition for a most general unifier. *)
 
-(* A Most General Unifier (MGU) takes in a term and a substitution and tells whether or not said substitution
-  is an mgu for the given term. *)
+(*  A Most General Unifier (MGU) takes in a term and a substitution and tells
+    whether or not said substitution is an mgu for the given term. *)
 Definition most_general_unifier (t : term) (s : subst) : Prop :=
-  (unifier t s) -> (forall (s' : subst), unifier t s' -> more_general_substitution s s' t ).
+  unifier t s ->
+  forall (s' : subst),
+  unifier t s' ->
+  more_general_substitution s s' t.
 
-(**
-  While this definition of a most general unifier is certainly valid, it is a somewhat unwieldy formulation. For this reason,
-let us now define an alternative definition called a reproductive unifier, and then prove it to be equivalent to
-our definition of a most general unifier. This will make our proofs easier to formulate down the road as the 
-task of proving a unifier to be reproductive is substantially easier than proving it to be most general directly. 
-**)
+(** While this definition of a most general unifier is certainly valid, it is a
+    somewhat unwieldy formulation. For this reason, let us now define an
+    alternative definition called a _reproductive unifier_, and then prove it to
+    be equivalent to our definition of a most general unifier. This will make
+    our proofs easier to formulate down the road as the task of proving a
+    unifier to be reproductive is substantially easier than proving it to be
+    most general directly. *)
 
 Definition reproductive_unifier (t : term) (sig : subst) : Prop :=
   unifier t sig ->
   forall (tau : subst) (x : var),
   unifier t tau ->
-  (apply_subst (apply_subst (VAR x) sig ) tau) == (apply_subst (VAR x) tau).
+  apply_subst (apply_subst (VAR x) sig ) tau == apply_subst (VAR x) tau.
 
 
 Lemma reproductive_is_mgu : forall (t : term) (u : subst),
   reproductive_unifier t u ->
   most_general_unifier t u.
 Proof.
- intros. unfold most_general_unifier.  unfold reproductive_unifier in H.
+  intros. unfold most_general_unifier. unfold reproductive_unifier in H.
   unfold more_general_substitution . unfold substitution_composition.
-  intros. specialize (H H0). exists s' . intros.  specialize (H s' x).  specialize (H H1). apply H.
+  intros. specialize (H H0). exists s'. intros. specialize (H s' x).
+  specialize (H H1). apply H.
 Qed.
 
 Lemma most_general_unifier_compat : forall  (t t' : term),
-     t == t' -> forall (sigma: subst), (most_general_unifier t sigma) <-> (most_general_unifier t' sigma).
+  t == t' ->
+  forall (sigma: subst),
+  most_general_unifier t sigma <-> most_general_unifier t' sigma.
 Proof.
-Admitted. 
+Admitted.
 
-(** * Auxilliary Computational Operations and Simplifications **)
+(** * Auxilliary Computational Operations and Simplifications *)
 
-(**
-These functions below will come in handy later during the Lowenheim formula proof. They mainly lay the 
-groundwork for providing the computational nuts and bolts for Lowenheim's algorithm for finding 
-most general unifiers.
-**)
+(** These functions below will come in handy later during the Lowenheim formula
+    proof. They mainly lay the groundwork for providing the computational nuts
+    and bolts for Lowenheim's algorithm for finding most general unifiers. *)
 
-(* alternate defintion of functions related to term operations and evaluations
-   that take into consideration more sub-cases *)
+(*  alternate defintion of functions related to term operations and evaluations
+    that take into consideration more sub-cases *)
 
-(* check if two terms are exaclty identical *)
+(*  check if two terms are exaclty identical *)
 Fixpoint identical (a b: term) : bool :=
   match a , b with
-    | T0, T0 => true
-    | T0, _ => false
-    | T1 , T1 => true
-    | T1 , _ => false
-    | VAR x , VAR y => if beq_nat x y then true else false
-    | VAR x, _ => false
-    | PRODUCT x y, PRODUCT x1 y1 => if ((identical x x1) && (identical y y1)) then true
-                                    else false
-    | PRODUCT x y, _ => false
-    | SUM x y, SUM x1 y1 => if ((identical x x1) && (identical y y1)) then true
-                                    else false
-    | SUM x y, _ => false
+  | T0, T0 => true
+  | T0, _ => false
+  | T1 , T1 => true
+  | T1 , _ => false
+  | VAR x , VAR y => if beq_nat x y then true else false
+  | VAR x, _ => false
+  | PRODUCT x y, PRODUCT x1 y1 => identical x x1 && identical y y1
+  | PRODUCT x y, _ => false
+  | SUM x y, SUM x1 y1 => identical x x1 && identical y y1
+  | SUM x y, _ => false
   end.
-    
 
-(* Basic Addition for terms *)
+
+(*  Basic Addition for terms *)
 Definition plus_one_step (a b : term) : term :=
   match a, b with
-    | T0, T0 => T0
-    | T0, T1 => T1
-    | T1, T0 => T1
-    | T1 , T1  => T0
-    | _ , _ => SUM a b
+  | T0, T0 => T0
+  | T0, T1 => T1
+  | T1, T0 => T1
+  | T1 , T1 => T0
+  | _ , _ => SUM a b
   end.
 
 
-(* Basic Multiplication for terms *)
+(*  Basic Multiplication for terms *)
 Definition mult_one_step (a b : term) : term :=
   match a, b with
-    | T0, T0 => T0
-    | T0, T1 => T0
-    | T1, T0 => T0
-    | T1 , T1  => T1
-    | _ , _ => PRODUCT a b
+  | T0, T0 => T0
+  | T0, T1 => T0
+  | T1, T0 => T0
+  | T1 , T1 => T1
+  | _ , _ => PRODUCT a b
   end.
 
 
-(* Simplifies a term in very apparent and basic ways *)
+(*  Simplifies a term in very apparent and basic ways *)
 Fixpoint simplify (t : term) : term :=
-  match t with 
-    | T0 => T0
-    | T1 => T1
-    | VAR x => VAR x (* T0 (* Set to 0 *) *)
-    | PRODUCT x y => mult_one_step (simplify x) (simplify y)
-    | SUM x y => plus_one_step (simplify x) (simplify y)
+  match t with
+  | T0 => T0
+  | T1 => T1
+  | VAR x => VAR x (* T0 (* Set to 0 *) *)
+  | PRODUCT x y => mult_one_step (simplify x) (simplify y)
+  | SUM x y => plus_one_step (simplify x) (simplify y)
   end.
 
 
-Lemma pos_left_sum_compat : forall  (t t1 t2 : term),
-     t == t1 -> plus_one_step t1 t2 == plus_one_step t t2. 
+Lemma pos_left_sum_compat : forall (t t1 t2 : term),
+  t == t1 -> plus_one_step t1 t2 == plus_one_step t t2.
 Proof.
   intros. induction t1.
   - induction t.
     + reflexivity.
     + apply T1_not_equiv_T0 in H. inversion H.
     + induction t2.
-      { simpl. rewrite H. rewrite sum_x_x. reflexivity. }
-      { simpl. rewrite H. rewrite sum_id. reflexivity. }
-      { simpl. rewrite H. reflexivity. }
-      { simpl. rewrite H. reflexivity. }
-      { simpl. rewrite H. reflexivity. }
+      * simpl. rewrite H. rewrite sum_x_x. reflexivity.
+      * simpl. rewrite H. rewrite sum_id. reflexivity.
+      * simpl. rewrite H. reflexivity.
+      * simpl. rewrite H. reflexivity.
+      * simpl. rewrite H. reflexivity.
     + induction t2.
-      { simpl. rewrite H. rewrite sum_x_x. reflexivity. }
-      { simpl. rewrite H. rewrite sum_id. reflexivity. }
-      { simpl. rewrite H. reflexivity. }
-      { simpl. rewrite H. reflexivity. }
-      { simpl. rewrite H. reflexivity. }
+      * simpl. rewrite H. rewrite sum_x_x. reflexivity.
+      * simpl. rewrite H. rewrite sum_id. reflexivity.
+      * simpl. rewrite H. reflexivity.
+      * simpl. rewrite H. reflexivity.
+      * simpl. rewrite H. reflexivity.
     + induction t2.
-      { simpl. rewrite H. rewrite sum_x_x. reflexivity. }
-      { simpl. rewrite H. rewrite sum_id. reflexivity. }
-      { simpl. rewrite H. reflexivity. }
-      { simpl. rewrite H. reflexivity. }
-      { simpl. rewrite H. reflexivity. }
+      * simpl. rewrite H. rewrite sum_x_x. reflexivity.
+      * simpl. rewrite H. rewrite sum_id. reflexivity.
+      * simpl. rewrite H. reflexivity.
+      * simpl. rewrite H. reflexivity.
+      * simpl. rewrite H. reflexivity.
   - induction t.
     + induction t2.
-      { simpl. rewrite H. reflexivity. }
-      { simpl. rewrite H. reflexivity. }
-      { simpl. rewrite H. reflexivity. }
-      { simpl. rewrite H. reflexivity. }
-      { simpl. rewrite H. reflexivity. }
+      * simpl. rewrite H. reflexivity.
+      * simpl. rewrite H. reflexivity.
+      * simpl. rewrite H. reflexivity.
+      * simpl. rewrite H. reflexivity.
+      * simpl. rewrite H. reflexivity.
     + induction t2.
-      { simpl. reflexivity. }
-      { simpl. reflexivity. }
-      { simpl. reflexivity. }
-      { simpl. reflexivity. }
-      { simpl. reflexivity. }
+      * simpl. reflexivity.
+      * simpl. reflexivity.
+      * simpl. reflexivity.
+      * simpl. reflexivity.
+      * simpl. reflexivity.
     + induction t2.
-      { simpl. rewrite H. rewrite sum_comm. rewrite sum_id. reflexivity. }
-      { simpl. rewrite H. rewrite sum_x_x. reflexivity. }
-      { simpl. rewrite H. reflexivity. }
-      { simpl. rewrite H. reflexivity. }
-      { simpl. rewrite H. reflexivity. }
+      * simpl. rewrite H. rewrite sum_comm. rewrite sum_id. reflexivity.
+      * simpl. rewrite H. rewrite sum_x_x. reflexivity.
+      * simpl. rewrite H. reflexivity.
+      * simpl. rewrite H. reflexivity.
+      * simpl. rewrite H. reflexivity.
     + induction t2.
-      { simpl. rewrite H. rewrite sum_comm. rewrite sum_id. reflexivity. }
-      { simpl. rewrite H. rewrite sum_x_x. reflexivity. }
-      { simpl. rewrite H. reflexivity. }
-      { simpl. rewrite H. reflexivity. }
-      { simpl. rewrite H. reflexivity. }
+      * simpl. rewrite H. rewrite sum_comm. rewrite sum_id. reflexivity.
+      * simpl. rewrite H. rewrite sum_x_x. reflexivity.
+      * simpl. rewrite H. reflexivity.
+      * simpl. rewrite H. reflexivity.
+      * simpl. rewrite H. reflexivity.
     + induction t2.
-      { simpl. rewrite H. rewrite sum_comm. rewrite sum_id. reflexivity. }
-      { simpl. rewrite H. rewrite sum_x_x. reflexivity. }
-      { simpl. rewrite H. reflexivity. }
-      { simpl. rewrite H. reflexivity. }
-      { simpl. rewrite H. reflexivity. }
+      * simpl. rewrite H. rewrite sum_comm. rewrite sum_id. reflexivity.
+      * simpl. rewrite H. rewrite sum_x_x. reflexivity.
+      * simpl. rewrite H. reflexivity.
+      * simpl. rewrite H. reflexivity.
+      * simpl. rewrite H. reflexivity.
   - induction t.
     + induction t2.
-      { simpl. rewrite H. rewrite sum_x_x. rewrite H. reflexivity. }
-      { simpl. rewrite <- H. rewrite sum_id. reflexivity. }
-      { simpl. rewrite H. reflexivity. }
-      { simpl. rewrite H. reflexivity. }
-      { simpl. rewrite H. reflexivity. }
+      * simpl. rewrite H. rewrite sum_x_x. rewrite H. reflexivity.
+      * simpl. rewrite <- H. rewrite sum_id. reflexivity.
+      * simpl. rewrite H. reflexivity.
+      * simpl. rewrite H. reflexivity.
+      * simpl. rewrite H. reflexivity.
     + induction t2.
-      { simpl. rewrite <- H. rewrite sum_comm. rewrite sum_id. reflexivity. }
-      { simpl. rewrite H. rewrite sum_x_x. reflexivity. }
-      { simpl. rewrite H. reflexivity. }
-      { simpl. rewrite H. reflexivity. }
-      { simpl. rewrite H. reflexivity. }
+      * simpl. rewrite <- H. rewrite sum_comm. rewrite sum_id. reflexivity.
+      * simpl. rewrite H. rewrite sum_x_x. reflexivity.
+      * simpl. rewrite H. reflexivity.
+      * simpl. rewrite H. reflexivity.
+      * simpl. rewrite H. reflexivity.
     + induction t2.
-      { simpl. rewrite H. reflexivity. }
-      { simpl. rewrite H. reflexivity. }
-      { simpl. rewrite H. reflexivity. }
-      { simpl. rewrite H. reflexivity. }
-      { simpl. rewrite H. reflexivity. }
+      * simpl. rewrite H. reflexivity.
+      * simpl. rewrite H. reflexivity.
+      * simpl. rewrite H. reflexivity.
+      * simpl. rewrite H. reflexivity.
+      * simpl. rewrite H. reflexivity.
     + induction t2.
-      { simpl. rewrite H. reflexivity. }
-      { simpl. rewrite H. reflexivity. }
-      { simpl. rewrite H. reflexivity. }
-      { simpl. rewrite H. reflexivity. }
-      { simpl. rewrite H. reflexivity. }
+      * simpl. rewrite H. reflexivity.
+      * simpl. rewrite H. reflexivity.
+      * simpl. rewrite H. reflexivity.
+      * simpl. rewrite H. reflexivity.
+      * simpl. rewrite H. reflexivity.
     + induction t2.
-      { simpl. rewrite H. reflexivity. }
-      { simpl. rewrite H. reflexivity. }
-      { simpl. rewrite H. reflexivity. }
-      { simpl. rewrite H. reflexivity. }
-      { simpl. rewrite H. reflexivity. } 
+      * simpl. rewrite H. reflexivity.
+      * simpl. rewrite H. reflexivity.
+      * simpl. rewrite H. reflexivity.
+      * simpl. rewrite H. reflexivity.
+      * simpl. rewrite H. reflexivity. 
   - induction t.
     + induction t2.
-      { simpl. rewrite <- H. rewrite sum_x_x. reflexivity. }
-      { simpl. rewrite <- H. rewrite sum_id. reflexivity. }
-      { simpl. rewrite <- H. reflexivity. }
-      { simpl. rewrite <- H. reflexivity. }
-      { simpl. rewrite <- H. reflexivity. }
+      * simpl. rewrite <- H. rewrite sum_x_x. reflexivity.
+      * simpl. rewrite <- H. rewrite sum_id. reflexivity.
+      * simpl. rewrite <- H. reflexivity.
+      * simpl. rewrite <- H. reflexivity.
+      * simpl. rewrite <- H. reflexivity.
     + induction t2.
-      { simpl. rewrite <- H. rewrite sum_comm. rewrite sum_id. reflexivity. }
-      { simpl. rewrite H. rewrite sum_x_x. reflexivity. }
-      { simpl. rewrite <- H. reflexivity. }
-      { simpl. rewrite <- H. reflexivity. }
-      { simpl. rewrite <- H. reflexivity. }
+      * simpl. rewrite <- H. rewrite sum_comm. rewrite sum_id. reflexivity.
+      * simpl. rewrite H. rewrite sum_x_x. reflexivity.
+      * simpl. rewrite <- H. reflexivity.
+      * simpl. rewrite <- H. reflexivity.
+      * simpl. rewrite <- H. reflexivity.
     + induction t2.
-      { simpl. rewrite H. reflexivity. }
-      { simpl. rewrite H. reflexivity. }
-      { simpl. rewrite H. reflexivity. }
-      { simpl. rewrite H. reflexivity. }
-      { simpl. rewrite H. reflexivity. }
+      * simpl. rewrite H. reflexivity.
+      * simpl. rewrite H. reflexivity.
+      * simpl. rewrite H. reflexivity.
+      * simpl. rewrite H. reflexivity.
+      * simpl. rewrite H. reflexivity.
     + induction t2.
-      { simpl. rewrite H. reflexivity. }
-      { simpl. rewrite H. reflexivity. }
-      { simpl. rewrite H. reflexivity. }
-      { simpl. rewrite H. reflexivity. }
-      { simpl. rewrite H. reflexivity. }
+      * simpl. rewrite H. reflexivity.
+      * simpl. rewrite H. reflexivity.
+      * simpl. rewrite H. reflexivity.
+      * simpl. rewrite H. reflexivity.
+      * simpl. rewrite H. reflexivity.
     + induction t2.
-      { simpl. rewrite H. reflexivity. }
-      { simpl. rewrite H. reflexivity. }
-      { simpl. rewrite H. reflexivity. }
-      { simpl. rewrite H. reflexivity. }
-      { simpl. rewrite H. reflexivity. }
+      * simpl. rewrite H. reflexivity.
+      * simpl. rewrite H. reflexivity.
+      * simpl. rewrite H. reflexivity.
+      * simpl. rewrite H. reflexivity.
+      * simpl. rewrite H. reflexivity.
  - induction t.
     + induction t2.
-      { simpl. rewrite <- H. rewrite sum_x_x. reflexivity. }
-      { simpl. rewrite <- H. rewrite sum_id. reflexivity. }
-      { simpl. rewrite <- H. reflexivity. }
-      { simpl. rewrite <- H. reflexivity. }
-      { simpl. rewrite <- H. reflexivity. }
+      * simpl. rewrite <- H. rewrite sum_x_x. reflexivity.
+      * simpl. rewrite <- H. rewrite sum_id. reflexivity.
+      * simpl. rewrite <- H. reflexivity.
+      * simpl. rewrite <- H. reflexivity.
+      * simpl. rewrite <- H. reflexivity.
     + induction t2.
-      { simpl. rewrite <- H. rewrite sum_comm. rewrite sum_id. reflexivity. }
-      { simpl. rewrite H. rewrite sum_x_x. reflexivity. }
-      { simpl. rewrite <- H. reflexivity. }
-      { simpl. rewrite <- H. reflexivity. }
-      { simpl. rewrite <- H. reflexivity. }
+      * simpl. rewrite <- H. rewrite sum_comm. rewrite sum_id. reflexivity.
+      * simpl. rewrite H. rewrite sum_x_x. reflexivity.
+      * simpl. rewrite <- H. reflexivity.
+      * simpl. rewrite <- H. reflexivity.
+      * simpl. rewrite <- H. reflexivity.
     + induction t2.
-      { simpl. rewrite H. reflexivity. }
-      { simpl. rewrite H. reflexivity. }
-      { simpl. rewrite H. reflexivity. }
-      { simpl. rewrite H. reflexivity. }
-      { simpl. rewrite H. reflexivity. }
+      * simpl. rewrite H. reflexivity.
+      * simpl. rewrite H. reflexivity.
+      * simpl. rewrite H. reflexivity.
+      * simpl. rewrite H. reflexivity.
+      * simpl. rewrite H. reflexivity.
     + induction t2.
-      { simpl. rewrite H. reflexivity. }
-      { simpl. rewrite H. reflexivity. }
-      { simpl. rewrite H. reflexivity. }
-      { simpl. rewrite H. reflexivity. }
-      { simpl. rewrite H. reflexivity. }
+      * simpl. rewrite H. reflexivity.
+      * simpl. rewrite H. reflexivity.
+      * simpl. rewrite H. reflexivity.
+      * simpl. rewrite H. reflexivity.
+      * simpl. rewrite H. reflexivity.
     + induction t2.
-      { simpl. rewrite H. reflexivity. }
-      { simpl. rewrite H. reflexivity. }
-      { simpl. rewrite H. reflexivity. }
-      { simpl. rewrite H. reflexivity. }
-      { simpl. rewrite H. reflexivity. }
+      * simpl. rewrite H. reflexivity.
+      * simpl. rewrite H. reflexivity.
+      * simpl. rewrite H. reflexivity.
+      * simpl. rewrite H. reflexivity.
+      * simpl. rewrite H. reflexivity.
 Qed.
 
 Lemma pos_right_sum_compat : forall  (t t1 t2 : term),
@@ -1208,159 +1161,159 @@ Proof.
 intros. induction t1.
   - induction t.
     + induction t2. 
-      { simpl. reflexivity. }
-      { simpl. rewrite H. reflexivity. }
-      { simpl. rewrite H. rewrite sum_x_x. apply H. }
-      { simpl. rewrite <- H. rewrite sum_x_x. reflexivity. }
-      { simpl. rewrite <- H. rewrite sum_x_x. reflexivity. }
+      * simpl. reflexivity.
+      * simpl. rewrite H. reflexivity.
+      * simpl. rewrite H. rewrite sum_x_x. apply H.
+      * simpl. rewrite <- H. rewrite sum_x_x. reflexivity.
+      * simpl. rewrite <- H. rewrite sum_x_x. reflexivity.
     + induction t2.
-      { simpl. rewrite H. reflexivity. }
-      { simpl. reflexivity. }
-      { simpl. rewrite H. rewrite sum_id. reflexivity. }
-      { simpl. rewrite H. rewrite sum_id. reflexivity. }
-      { simpl. rewrite <- H. rewrite sum_id. reflexivity. }
+      * simpl. rewrite H. reflexivity.
+      * simpl. reflexivity.
+      * simpl. rewrite H. rewrite sum_id. reflexivity.
+      * simpl. rewrite H. rewrite sum_id. reflexivity.
+      * simpl. rewrite <- H. rewrite sum_id. reflexivity.
     + induction t2.
-      { simpl. rewrite H. rewrite sum_x_x. reflexivity. }
-      { simpl. rewrite H. rewrite sum_id. reflexivity. }
-      { simpl. rewrite H. rewrite sum_id. reflexivity. }
-      { simpl. rewrite H. rewrite sum_id. reflexivity. }
-      { simpl. rewrite <- H. rewrite sum_id. reflexivity. }
+      * simpl. rewrite H. rewrite sum_x_x. reflexivity.
+      * simpl. rewrite H. rewrite sum_id. reflexivity.
+      * simpl. rewrite H. rewrite sum_id. reflexivity.
+      * simpl. rewrite H. rewrite sum_id. reflexivity.
+      * simpl. rewrite <- H. rewrite sum_id. reflexivity.
     + induction t2.
-      { simpl. rewrite H. rewrite sum_x_x. reflexivity. }
-      { simpl. rewrite H. rewrite sum_id. reflexivity. }
-      { simpl. rewrite H. rewrite sum_id. reflexivity. }
-      { simpl. rewrite H. rewrite sum_id. reflexivity. }
-      { simpl. rewrite <- H. rewrite sum_id. reflexivity. }
+      * simpl. rewrite H. rewrite sum_x_x. reflexivity.
+      * simpl. rewrite H. rewrite sum_id. reflexivity.
+      * simpl. rewrite H. rewrite sum_id. reflexivity.
+      * simpl. rewrite H. rewrite sum_id. reflexivity.
+      * simpl. rewrite <- H. rewrite sum_id. reflexivity.
     + induction t2.
-      { simpl. rewrite H. rewrite sum_x_x. reflexivity. }
-      { simpl. rewrite H. rewrite sum_id. reflexivity. }
-      { simpl. rewrite H. rewrite sum_id. reflexivity. }
-      { simpl. rewrite H. rewrite sum_id. reflexivity. }
-      { simpl. rewrite <- H. rewrite sum_id. reflexivity. }
+      * simpl. rewrite H. rewrite sum_x_x. reflexivity.
+      * simpl. rewrite H. rewrite sum_id. reflexivity.
+      * simpl. rewrite H. rewrite sum_id. reflexivity.
+      * simpl. rewrite H. rewrite sum_id. reflexivity.
+      * simpl. rewrite <- H. rewrite sum_id. reflexivity.
   - induction t.
     + induction t2. 
-      { simpl. reflexivity. }
-      { simpl. rewrite H. reflexivity. }
-      { simpl. rewrite <- H. rewrite sum_comm. rewrite sum_id. reflexivity. }
-      { simpl. rewrite <- H. rewrite sum_comm. rewrite sum_id. reflexivity. }
-      { simpl. rewrite <- H. rewrite sum_comm. rewrite sum_id. reflexivity. }
+      * simpl. reflexivity.
+      * simpl. rewrite H. reflexivity.
+      * simpl. rewrite <- H. rewrite sum_comm. rewrite sum_id. reflexivity.
+      * simpl. rewrite <- H. rewrite sum_comm. rewrite sum_id. reflexivity.
+      * simpl. rewrite <- H. rewrite sum_comm. rewrite sum_id. reflexivity.
     + induction t2.
-      { simpl. rewrite H. reflexivity. }
-      { simpl. reflexivity. }
-      { simpl. rewrite H. rewrite sum_x_x. reflexivity. }
-      { simpl. rewrite H. rewrite sum_x_x. reflexivity. }
-      { simpl. rewrite <- H. rewrite sum_x_x. reflexivity. }
+      * simpl. rewrite H. reflexivity.
+      * simpl. reflexivity.
+      * simpl. rewrite H. rewrite sum_x_x. reflexivity.
+      * simpl. rewrite H. rewrite sum_x_x. reflexivity.
+      * simpl. rewrite <- H. rewrite sum_x_x. reflexivity.
     + induction t2.
-      { simpl. rewrite H. rewrite sum_comm. rewrite sum_id. reflexivity. }
-      { simpl. rewrite H. rewrite sum_x_x. reflexivity. }
-      { simpl. rewrite H. reflexivity. }
-      { simpl. rewrite H. reflexivity. }
-      { simpl. rewrite <- H. reflexivity. }
+      * simpl. rewrite H. rewrite sum_comm. rewrite sum_id. reflexivity.
+      * simpl. rewrite H. rewrite sum_x_x. reflexivity.
+      * simpl. rewrite H. reflexivity.
+      * simpl. rewrite H. reflexivity.
+      * simpl. rewrite <- H. reflexivity.
     + induction t2.
-      { simpl. rewrite H. rewrite sum_comm. rewrite sum_id. reflexivity. }
-      { simpl. rewrite H. rewrite sum_x_x. reflexivity. }
-      { simpl. rewrite H. reflexivity. }
-      { simpl. rewrite H. reflexivity. }
-      { simpl. rewrite <- H. reflexivity. }
+      * simpl. rewrite H. rewrite sum_comm. rewrite sum_id. reflexivity.
+      * simpl. rewrite H. rewrite sum_x_x. reflexivity.
+      * simpl. rewrite H. reflexivity.
+      * simpl. rewrite H. reflexivity.
+      * simpl. rewrite <- H. reflexivity.
     + induction t2.
-      { simpl. rewrite H. rewrite sum_comm. rewrite sum_id. reflexivity. }
-      { simpl. rewrite H. rewrite sum_x_x. reflexivity. }
-      { simpl. rewrite H. reflexivity. }
-      { simpl. rewrite H. reflexivity. }
-      { simpl. rewrite <- H. reflexivity. }
+      * simpl. rewrite H. rewrite sum_comm. rewrite sum_id. reflexivity.
+      * simpl. rewrite H. rewrite sum_x_x. reflexivity.
+      * simpl. rewrite H. reflexivity.
+      * simpl. rewrite H. reflexivity.
+      * simpl. rewrite <- H. reflexivity.
   - induction t.
     + induction t2. 
-      { simpl. reflexivity. }
-      { simpl. rewrite H. reflexivity. }
-      { simpl. rewrite <- H. reflexivity. }
-      { simpl. rewrite <- H. reflexivity. }
-      { simpl. rewrite <- H. reflexivity. }
+      * simpl. reflexivity.
+      * simpl. rewrite H. reflexivity.
+      * simpl. rewrite <- H. reflexivity.
+      * simpl. rewrite <- H. reflexivity.
+      * simpl. rewrite <- H. reflexivity.
     + induction t2.
-      { simpl. rewrite H. reflexivity. }
-      { simpl. reflexivity. }
-      { simpl. rewrite H. reflexivity. }
-      { simpl. rewrite H. reflexivity. }
-      { simpl. rewrite <- H. reflexivity. }
+      * simpl. rewrite H. reflexivity.
+      * simpl. reflexivity.
+      * simpl. rewrite H. reflexivity.
+      * simpl. rewrite H. reflexivity.
+      * simpl. rewrite <- H. reflexivity.
     + induction t2.
-      { simpl. rewrite H. reflexivity. }
-      { simpl. rewrite H. reflexivity. }
-      { simpl. rewrite H. reflexivity. }
-      { simpl. rewrite H. reflexivity. }
-      { simpl. rewrite <- H. reflexivity. }
+      * simpl. rewrite H. reflexivity.
+      * simpl. rewrite H. reflexivity.
+      * simpl. rewrite H. reflexivity.
+      * simpl. rewrite H. reflexivity.
+      * simpl. rewrite <- H. reflexivity.
     + induction t2.
-      { simpl. rewrite H. reflexivity. }
-      { simpl. rewrite H. reflexivity. }
-      { simpl. rewrite H. reflexivity. }
-      { simpl. rewrite H. reflexivity. }
-      { simpl. rewrite <- H. reflexivity. }
+      * simpl. rewrite H. reflexivity.
+      * simpl. rewrite H. reflexivity.
+      * simpl. rewrite H. reflexivity.
+      * simpl. rewrite H. reflexivity.
+      * simpl. rewrite <- H. reflexivity.
     + induction t2.
-      { simpl. rewrite H. reflexivity. }
-      { simpl. rewrite H. reflexivity. }
-      { simpl. rewrite H. reflexivity. }
-      { simpl. rewrite H. reflexivity. }
-      { simpl. rewrite <- H. reflexivity. }
+      * simpl. rewrite H. reflexivity.
+      * simpl. rewrite H. reflexivity.
+      * simpl. rewrite H. reflexivity.
+      * simpl. rewrite H. reflexivity.
+      * simpl. rewrite <- H. reflexivity.
   - induction t.
     + induction t2. 
-      { simpl. reflexivity. }
-      { simpl. rewrite H. reflexivity. }
-      { simpl. rewrite <- H. reflexivity. }
-      { simpl. rewrite <- H. reflexivity. }
-      { simpl. rewrite <- H. reflexivity. }
+      * simpl. reflexivity.
+      * simpl. rewrite H. reflexivity.
+      * simpl. rewrite <- H. reflexivity.
+      * simpl. rewrite <- H. reflexivity.
+      * simpl. rewrite <- H. reflexivity.
     + induction t2.
-      { simpl. rewrite H. reflexivity. }
-      { simpl. reflexivity. }
-      { simpl. rewrite H. reflexivity. }
-      { simpl. rewrite H. reflexivity. }
-      { simpl. rewrite <- H. reflexivity. }
+      * simpl. rewrite H. reflexivity.
+      * simpl. reflexivity.
+      * simpl. rewrite H. reflexivity.
+      * simpl. rewrite H. reflexivity.
+      * simpl. rewrite <- H. reflexivity.
     + induction t2.
-      { simpl. rewrite H. reflexivity. }
-      { simpl. rewrite H. reflexivity. }
-      { simpl. rewrite H. reflexivity. }
-      { simpl. rewrite H. reflexivity. }
-      { simpl. rewrite <- H. reflexivity. }
+      * simpl. rewrite H. reflexivity.
+      * simpl. rewrite H. reflexivity.
+      * simpl. rewrite H. reflexivity.
+      * simpl. rewrite H. reflexivity.
+      * simpl. rewrite <- H. reflexivity.
     + induction t2.
-      { simpl. rewrite H. reflexivity. }
-      { simpl. rewrite H. reflexivity. }
-      { simpl. rewrite H. reflexivity. }
-      { simpl. rewrite H. reflexivity. }
-      { simpl. rewrite <- H. reflexivity. }
+      * simpl. rewrite H. reflexivity.
+      * simpl. rewrite H. reflexivity.
+      * simpl. rewrite H. reflexivity.
+      * simpl. rewrite H. reflexivity.
+      * simpl. rewrite <- H. reflexivity.
     + induction t2.
-      { simpl. rewrite H. reflexivity. }
-      { simpl. rewrite H. reflexivity. }
-      { simpl. rewrite H. reflexivity. }
-      { simpl. rewrite H. reflexivity. }
-      { simpl. rewrite <- H. reflexivity. }
+      * simpl. rewrite H. reflexivity.
+      * simpl. rewrite H. reflexivity.
+      * simpl. rewrite H. reflexivity.
+      * simpl. rewrite H. reflexivity.
+      * simpl. rewrite <- H. reflexivity.
   - induction t.
     + induction t2. 
-      { simpl. reflexivity. }
-      { simpl. rewrite H. reflexivity. }
-      { simpl. rewrite <- H. reflexivity. }
-      { simpl. rewrite <- H. reflexivity. }
-      { simpl. rewrite <- H. reflexivity. }
+      * simpl. reflexivity.
+      * simpl. rewrite H. reflexivity.
+      * simpl. rewrite <- H. reflexivity.
+      * simpl. rewrite <- H. reflexivity.
+      * simpl. rewrite <- H. reflexivity.
     + induction t2.
-      { simpl. rewrite H. reflexivity. }
-      { simpl. reflexivity. }
-      { simpl. rewrite H. reflexivity. }
-      { simpl. rewrite H. reflexivity. }
-      { simpl. rewrite <- H. reflexivity. }
+      * simpl. rewrite H. reflexivity.
+      * simpl. reflexivity.
+      * simpl. rewrite H. reflexivity.
+      * simpl. rewrite H. reflexivity.
+      * simpl. rewrite <- H. reflexivity.
     + induction t2.
-      { simpl. rewrite H. reflexivity. }
-      { simpl. rewrite H. reflexivity. }
-      { simpl. rewrite H. reflexivity. }
-      { simpl. rewrite H. reflexivity. }
-      { simpl. rewrite <- H. reflexivity. }
+      * simpl. rewrite H. reflexivity.
+      * simpl. rewrite H. reflexivity.
+      * simpl. rewrite H. reflexivity.
+      * simpl. rewrite H. reflexivity.
+      * simpl. rewrite <- H. reflexivity.
     + induction t2.
-      { simpl. rewrite H. reflexivity. }
-      { simpl. rewrite H. reflexivity. }
-      { simpl. rewrite H. reflexivity. }
-      { simpl. rewrite H. reflexivity. }
-      { simpl. rewrite <- H. reflexivity. }
+      * simpl. rewrite H. reflexivity.
+      * simpl. rewrite H. reflexivity.
+      * simpl. rewrite H. reflexivity.
+      * simpl. rewrite H. reflexivity.
+      * simpl. rewrite <- H. reflexivity.
     + induction t2.
-      { simpl. rewrite H. reflexivity. }
-      { simpl. rewrite H. reflexivity. }
-      { simpl. rewrite H. reflexivity. }
-      { simpl. rewrite H. reflexivity. }
-      { simpl. rewrite <- H. reflexivity. }
+      * simpl. rewrite H. reflexivity.
+      * simpl. rewrite H. reflexivity.
+      * simpl. rewrite H. reflexivity.
+      * simpl. rewrite H. reflexivity.
+      * simpl. rewrite <- H. reflexivity.
 Qed.
 
 Lemma pos_left_mul_compat : forall  (t t1 t2 : term),
@@ -1371,147 +1324,147 @@ Proof.
     + reflexivity.
     + apply T1_not_equiv_T0 in H. inversion H.
     + induction t2.
-      { simpl. rewrite H. rewrite mul_x_x. reflexivity. }
-      { simpl. rewrite H. rewrite mul_T0_x. reflexivity. }
-      { simpl. rewrite H. reflexivity. }
-      { simpl. rewrite H. reflexivity. }
-      { simpl. rewrite H. reflexivity. }
+      * simpl. rewrite H. rewrite mul_x_x. reflexivity.
+      * simpl. rewrite H. rewrite mul_T0_x. reflexivity.
+      * simpl. rewrite H. reflexivity.
+      * simpl. rewrite H. reflexivity.
+      * simpl. rewrite H. reflexivity.
     + induction t2.
-      { simpl. rewrite H. rewrite mul_x_x. reflexivity. }
-      { simpl. rewrite H. rewrite mul_T0_x. reflexivity. }
-      { simpl. rewrite H. reflexivity. }
-      { simpl. rewrite H. reflexivity. }
-      { simpl. rewrite H. reflexivity. }
+      * simpl. rewrite H. rewrite mul_x_x. reflexivity.
+      * simpl. rewrite H. rewrite mul_T0_x. reflexivity.
+      * simpl. rewrite H. reflexivity.
+      * simpl. rewrite H. reflexivity.
+      * simpl. rewrite H. reflexivity.
     + induction t2.
-      { simpl. rewrite H. rewrite mul_x_x. reflexivity. }
-      { simpl. rewrite H. rewrite mul_T0_x. reflexivity. }
-      { simpl. rewrite H. reflexivity. }
-      { simpl. rewrite H. reflexivity. }
-      { simpl. rewrite H. reflexivity. }
+      * simpl. rewrite H. rewrite mul_x_x. reflexivity.
+      * simpl. rewrite H. rewrite mul_T0_x. reflexivity.
+      * simpl. rewrite H. reflexivity.
+      * simpl. rewrite H. reflexivity.
+      * simpl. rewrite H. reflexivity.
   - induction t.
     + induction t2.
-      { simpl. rewrite H. reflexivity. }
-      { simpl. rewrite H. reflexivity. }
-      { simpl. rewrite H. reflexivity. }
-      { simpl. rewrite H. reflexivity. }
-      { simpl. rewrite H. reflexivity. }
+      * simpl. rewrite H. reflexivity.
+      * simpl. rewrite H. reflexivity.
+      * simpl. rewrite H. reflexivity.
+      * simpl. rewrite H. reflexivity.
+      * simpl. rewrite H. reflexivity.
     + induction t2.
-      { simpl. reflexivity. }
-      { simpl. reflexivity. }
-      { simpl. reflexivity. }
-      { simpl. reflexivity. }
-      { simpl. reflexivity. }
+      * simpl. reflexivity.
+      * simpl. reflexivity.
+      * simpl. reflexivity.
+      * simpl. reflexivity.
+      * simpl. reflexivity.
     + induction t2.
-      { simpl. rewrite H. rewrite mul_comm. rewrite mul_T0_x. reflexivity. }
-      { simpl. rewrite H. rewrite mul_x_x. reflexivity. }
-      { simpl. rewrite H. reflexivity. }
-      { simpl. rewrite H. reflexivity. }
-      { simpl. rewrite H. reflexivity. }
+      * simpl. rewrite H. rewrite mul_comm. rewrite mul_T0_x. reflexivity.
+      * simpl. rewrite H. rewrite mul_x_x. reflexivity.
+      * simpl. rewrite H. reflexivity.
+      * simpl. rewrite H. reflexivity.
+      * simpl. rewrite H. reflexivity.
     + induction t2.
-      { simpl. rewrite H. rewrite mul_comm. rewrite mul_T0_x. reflexivity. }
-      { simpl. rewrite H. rewrite mul_x_x. reflexivity. }
-      { simpl. rewrite H. reflexivity. }
-      { simpl. rewrite H. reflexivity. }
-      { simpl. rewrite H. reflexivity. }
+      * simpl. rewrite H. rewrite mul_comm. rewrite mul_T0_x. reflexivity.
+      * simpl. rewrite H. rewrite mul_x_x. reflexivity.
+      * simpl. rewrite H. reflexivity.
+      * simpl. rewrite H. reflexivity.
+      * simpl. rewrite H. reflexivity.
     + induction t2.
-      { simpl. rewrite H. rewrite mul_comm. rewrite mul_T0_x. reflexivity. }
-      { simpl. rewrite H. rewrite mul_x_x. reflexivity. }
-      { simpl. rewrite H. reflexivity. }
-      { simpl. rewrite H. reflexivity. }
-      { simpl. rewrite H. reflexivity. }
+      * simpl. rewrite H. rewrite mul_comm. rewrite mul_T0_x. reflexivity.
+      * simpl. rewrite H. rewrite mul_x_x. reflexivity.
+      * simpl. rewrite H. reflexivity.
+      * simpl. rewrite H. reflexivity.
+      * simpl. rewrite H. reflexivity.
   - induction t.
     + induction t2.
-      { simpl. rewrite H. rewrite mul_x_x. reflexivity. }
-      { simpl. rewrite <- H. rewrite mul_T0_x. reflexivity. }
-      { simpl. rewrite H. reflexivity. }
-      { simpl. rewrite H. reflexivity. }
-      { simpl. rewrite H. reflexivity. }
+      * simpl. rewrite H. rewrite mul_x_x. reflexivity.
+      * simpl. rewrite <- H. rewrite mul_T0_x. reflexivity.
+      * simpl. rewrite H. reflexivity.
+      * simpl. rewrite H. reflexivity.
+      * simpl. rewrite H. reflexivity.
     + induction t2.
-      { simpl. rewrite <- H. rewrite mul_comm. rewrite mul_T0_x. reflexivity. }
-      { simpl. rewrite H. rewrite mul_x_x. reflexivity. }
-      { simpl. rewrite H. reflexivity. }
-      { simpl. rewrite H. reflexivity. }
-      { simpl. rewrite H. reflexivity. }
+      * simpl. rewrite <- H. rewrite mul_comm. rewrite mul_T0_x. reflexivity.
+      * simpl. rewrite H. rewrite mul_x_x. reflexivity.
+      * simpl. rewrite H. reflexivity.
+      * simpl. rewrite H. reflexivity.
+      * simpl. rewrite H. reflexivity.
     + induction t2.
-      { simpl. rewrite H. reflexivity. }
-      { simpl. rewrite H. reflexivity. }
-      { simpl. rewrite H. reflexivity. }
-      { simpl. rewrite H. reflexivity. }
-      { simpl. rewrite H. reflexivity. }
+      * simpl. rewrite H. reflexivity.
+      * simpl. rewrite H. reflexivity.
+      * simpl. rewrite H. reflexivity.
+      * simpl. rewrite H. reflexivity.
+      * simpl. rewrite H. reflexivity.
     + induction t2.
-      { simpl. rewrite H. reflexivity. }
-      { simpl. rewrite H. reflexivity. }
-      { simpl. rewrite H. reflexivity. }
-      { simpl. rewrite H. reflexivity. }
-      { simpl. rewrite H. reflexivity. }
+      * simpl. rewrite H. reflexivity.
+      * simpl. rewrite H. reflexivity.
+      * simpl. rewrite H. reflexivity.
+      * simpl. rewrite H. reflexivity.
+      * simpl. rewrite H. reflexivity.
     + induction t2.
-      { simpl. rewrite H. reflexivity. }
-      { simpl. rewrite H. reflexivity. }
-      { simpl. rewrite H. reflexivity. }
-      { simpl. rewrite H. reflexivity. }
-      { simpl. rewrite H. reflexivity. } 
+      * simpl. rewrite H. reflexivity.
+      * simpl. rewrite H. reflexivity.
+      * simpl. rewrite H. reflexivity.
+      * simpl. rewrite H. reflexivity.
+      * simpl. rewrite H. reflexivity. 
   - induction t.
     + induction t2.
-      { simpl. rewrite <- H. rewrite mul_x_x. reflexivity. }
-      { simpl. rewrite <- H. rewrite mul_T0_x. reflexivity. }
-      { simpl. rewrite <- H. reflexivity. }
-      { simpl. rewrite <- H. reflexivity. }
-      { simpl. rewrite <- H. reflexivity. }
+      * simpl. rewrite <- H. rewrite mul_x_x. reflexivity.
+      * simpl. rewrite <- H. rewrite mul_T0_x. reflexivity.
+      * simpl. rewrite <- H. reflexivity.
+      * simpl. rewrite <- H. reflexivity.
+      * simpl. rewrite <- H. reflexivity.
     + induction t2.
-      { simpl. rewrite <- H. rewrite mul_comm. rewrite mul_T0_x. reflexivity. }
-      { simpl. rewrite H. rewrite mul_x_x. reflexivity. }
-      { simpl. rewrite <- H. reflexivity. }
-      { simpl. rewrite <- H. reflexivity. }
-      { simpl. rewrite <- H. reflexivity. }
+      * simpl. rewrite <- H. rewrite mul_comm. rewrite mul_T0_x. reflexivity.
+      * simpl. rewrite H. rewrite mul_x_x. reflexivity.
+      * simpl. rewrite <- H. reflexivity.
+      * simpl. rewrite <- H. reflexivity.
+      * simpl. rewrite <- H. reflexivity.
     + induction t2.
-      { simpl. rewrite H. reflexivity. }
-      { simpl. rewrite H. reflexivity. }
-      { simpl. rewrite H. reflexivity. }
-      { simpl. rewrite H. reflexivity. }
-      { simpl. rewrite H. reflexivity. }
+      * simpl. rewrite H. reflexivity.
+      * simpl. rewrite H. reflexivity.
+      * simpl. rewrite H. reflexivity.
+      * simpl. rewrite H. reflexivity.
+      * simpl. rewrite H. reflexivity.
     + induction t2.
-      { simpl. rewrite H. reflexivity. }
-      { simpl. rewrite H. reflexivity. }
-      { simpl. rewrite H. reflexivity. }
-      { simpl. rewrite H. reflexivity. }
-      { simpl. rewrite H. reflexivity. }
+      * simpl. rewrite H. reflexivity.
+      * simpl. rewrite H. reflexivity.
+      * simpl. rewrite H. reflexivity.
+      * simpl. rewrite H. reflexivity.
+      * simpl. rewrite H. reflexivity.
     + induction t2.
-      { simpl. rewrite H. reflexivity. }
-      { simpl. rewrite H. reflexivity. }
-      { simpl. rewrite H. reflexivity. }
-      { simpl. rewrite H. reflexivity. }
-      { simpl. rewrite H. reflexivity. }
+      * simpl. rewrite H. reflexivity.
+      * simpl. rewrite H. reflexivity.
+      * simpl. rewrite H. reflexivity.
+      * simpl. rewrite H. reflexivity.
+      * simpl. rewrite H. reflexivity.
   - induction t.
     + induction t2.
-      { simpl. rewrite <- H. rewrite mul_x_x. reflexivity. }
-      { simpl. rewrite <- H. rewrite mul_T0_x. reflexivity. }
-      { simpl. rewrite <- H. reflexivity. }
-      { simpl. rewrite <- H. reflexivity. }
-      { simpl. rewrite <- H. reflexivity. }
+      * simpl. rewrite <- H. rewrite mul_x_x. reflexivity.
+      * simpl. rewrite <- H. rewrite mul_T0_x. reflexivity.
+      * simpl. rewrite <- H. reflexivity.
+      * simpl. rewrite <- H. reflexivity.
+      * simpl. rewrite <- H. reflexivity.
     + induction t2.
-      { simpl. rewrite <- H. rewrite mul_comm. rewrite mul_T0_x. reflexivity. }
-      { simpl. rewrite H. rewrite mul_x_x. reflexivity. }
-      { simpl. rewrite <- H. reflexivity. }
-      { simpl. rewrite <- H. reflexivity. }
-      { simpl. rewrite <- H. reflexivity. }
+      * simpl. rewrite <- H. rewrite mul_comm. rewrite mul_T0_x. reflexivity.
+      * simpl. rewrite H. rewrite mul_x_x. reflexivity.
+      * simpl. rewrite <- H. reflexivity.
+      * simpl. rewrite <- H. reflexivity.
+      * simpl. rewrite <- H. reflexivity.
     + induction t2.
-      { simpl. rewrite H. reflexivity. }
-      { simpl. rewrite H. reflexivity. }
-      { simpl. rewrite H. reflexivity. }
-      { simpl. rewrite H. reflexivity. }
-      { simpl. rewrite H. reflexivity. }
+      * simpl. rewrite H. reflexivity.
+      * simpl. rewrite H. reflexivity.
+      * simpl. rewrite H. reflexivity.
+      * simpl. rewrite H. reflexivity.
+      * simpl. rewrite H. reflexivity.
     + induction t2.
-      { simpl. rewrite H. reflexivity. }
-      { simpl. rewrite H. reflexivity. }
-      { simpl. rewrite H. reflexivity. }
-      { simpl. rewrite H. reflexivity. }
-      { simpl. rewrite H. reflexivity. }
+      * simpl. rewrite H. reflexivity.
+      * simpl. rewrite H. reflexivity.
+      * simpl. rewrite H. reflexivity.
+      * simpl. rewrite H. reflexivity.
+      * simpl. rewrite H. reflexivity.
     + induction t2.
-      { simpl. rewrite H. reflexivity. }
-      { simpl. rewrite H. reflexivity. }
-      { simpl. rewrite H. reflexivity. }
-      { simpl. rewrite H. reflexivity. }
-      { simpl. rewrite H. reflexivity. }
+      * simpl. rewrite H. reflexivity.
+      * simpl. rewrite H. reflexivity.
+      * simpl. rewrite H. reflexivity.
+      * simpl. rewrite H. reflexivity.
+      * simpl. rewrite H. reflexivity.
 Qed.
 
 Lemma pos_right_mul_compat : forall  (t t1 t2 : term),
@@ -1520,214 +1473,214 @@ Proof.
 intros. induction t1.
   - induction t.
     + induction t2. 
-      { simpl. reflexivity. }
-      { simpl. rewrite H. reflexivity. }
-      { simpl. rewrite H. rewrite mul_x_x. reflexivity. }
-      { simpl. rewrite <- H. rewrite mul_x_x. reflexivity. }
-      { simpl. rewrite <- H. rewrite mul_x_x. reflexivity. }
+      * simpl. reflexivity.
+      * simpl. rewrite H. reflexivity.
+      * simpl. rewrite H. rewrite mul_x_x. reflexivity.
+      * simpl. rewrite <- H. rewrite mul_x_x. reflexivity.
+      * simpl. rewrite <- H. rewrite mul_x_x. reflexivity.
     + induction t2.
-      { simpl. reflexivity. }
-      { simpl. reflexivity. }
-      { simpl. rewrite mul_T0_x. reflexivity. }
-      { simpl. rewrite mul_T0_x. reflexivity. }
-      { simpl. rewrite mul_T0_x. reflexivity. }
+      * simpl. reflexivity.
+      * simpl. reflexivity.
+      * simpl. rewrite mul_T0_x. reflexivity.
+      * simpl. rewrite mul_T0_x. reflexivity.
+      * simpl. rewrite mul_T0_x. reflexivity.
     + induction t2.
-      { simpl. rewrite mul_T0_x. reflexivity. }
-      { simpl. rewrite mul_T0_x. reflexivity. }
-      { simpl. rewrite mul_T0_x. rewrite mul_T0_x. reflexivity. }
-      { simpl. rewrite mul_T0_x. rewrite mul_T0_x. reflexivity. }
-      { simpl. rewrite mul_T0_x. rewrite mul_T0_x. reflexivity. }
+      * simpl. rewrite mul_T0_x. reflexivity.
+      * simpl. rewrite mul_T0_x. reflexivity.
+      * simpl. rewrite mul_T0_x. rewrite mul_T0_x. reflexivity.
+      * simpl. rewrite mul_T0_x. rewrite mul_T0_x. reflexivity.
+      * simpl. rewrite mul_T0_x. rewrite mul_T0_x. reflexivity.
     + induction t2.
-      { simpl. rewrite mul_T0_x. reflexivity. }
-      { simpl. rewrite mul_T0_x. reflexivity. }
-      { simpl. rewrite mul_T0_x. rewrite mul_T0_x. reflexivity. }
-      { simpl. rewrite mul_T0_x. rewrite mul_T0_x. reflexivity. }
-      { simpl. rewrite mul_T0_x. rewrite mul_T0_x. reflexivity. }
+      * simpl. rewrite mul_T0_x. reflexivity.
+      * simpl. rewrite mul_T0_x. reflexivity.
+      * simpl. rewrite mul_T0_x. rewrite mul_T0_x. reflexivity.
+      * simpl. rewrite mul_T0_x. rewrite mul_T0_x. reflexivity.
+      * simpl. rewrite mul_T0_x. rewrite mul_T0_x. reflexivity.
     + induction t2.
-      { simpl. rewrite mul_T0_x. reflexivity. }
-      { simpl. rewrite mul_T0_x. reflexivity. }
-      { simpl. rewrite mul_T0_x. rewrite mul_T0_x. reflexivity. }
-      { simpl. rewrite mul_T0_x. rewrite mul_T0_x. reflexivity. }
-      { simpl. rewrite mul_T0_x. rewrite mul_T0_x. reflexivity. }
+      * simpl. rewrite mul_T0_x. reflexivity.
+      * simpl. rewrite mul_T0_x. reflexivity.
+      * simpl. rewrite mul_T0_x. rewrite mul_T0_x. reflexivity.
+      * simpl. rewrite mul_T0_x. rewrite mul_T0_x. reflexivity.
+      * simpl. rewrite mul_T0_x. rewrite mul_T0_x. reflexivity.
   - induction t.
     + induction t2. 
-      { simpl. reflexivity. }
-      { simpl. rewrite H. reflexivity. }
-      { simpl. rewrite <- H. rewrite mul_comm. rewrite mul_T0_x. reflexivity. }
-      { simpl. rewrite <- H. rewrite mul_comm. rewrite mul_T0_x. reflexivity. }
-      { simpl. rewrite <- H. rewrite mul_comm. rewrite mul_T0_x. reflexivity. }
+      * simpl. reflexivity.
+      * simpl. rewrite H. reflexivity.
+      * simpl. rewrite <- H. rewrite mul_comm. rewrite mul_T0_x. reflexivity.
+      * simpl. rewrite <- H. rewrite mul_comm. rewrite mul_T0_x. reflexivity.
+      * simpl. rewrite <- H. rewrite mul_comm. rewrite mul_T0_x. reflexivity.
     + induction t2.
-      { simpl. rewrite H. reflexivity. }
-      { simpl. reflexivity. }
-      { simpl. rewrite H. rewrite mul_x_x. reflexivity. }
-      { simpl. rewrite H. rewrite mul_x_x. reflexivity. }
-      { simpl. rewrite <- H. rewrite mul_x_x. reflexivity. }
+      * simpl. rewrite H. reflexivity.
+      * simpl. reflexivity.
+      * simpl. rewrite H. rewrite mul_x_x. reflexivity.
+      * simpl. rewrite H. rewrite mul_x_x. reflexivity.
+      * simpl. rewrite <- H. rewrite mul_x_x. reflexivity.
     + induction t2.
-      { simpl. rewrite H. rewrite mul_comm. rewrite mul_T0_x. reflexivity. }
-      { simpl. rewrite H. rewrite mul_x_x. reflexivity. }
-      { simpl. rewrite H. reflexivity. }
-      { simpl. rewrite H. reflexivity. }
-      { simpl. rewrite <- H. reflexivity. }
+      * simpl. rewrite H. rewrite mul_comm. rewrite mul_T0_x. reflexivity.
+      * simpl. rewrite H. rewrite mul_x_x. reflexivity.
+      * simpl. rewrite H. reflexivity.
+      * simpl. rewrite H. reflexivity.
+      * simpl. rewrite <- H. reflexivity.
     + induction t2.
-      { simpl. rewrite H. rewrite mul_comm. rewrite mul_T0_x. reflexivity. }
-      { simpl. rewrite H. rewrite mul_x_x. reflexivity. }
-      { simpl. rewrite H. reflexivity. }
-      { simpl. rewrite H. reflexivity. }
-      { simpl. rewrite <- H. reflexivity. }
+      * simpl. rewrite H. rewrite mul_comm. rewrite mul_T0_x. reflexivity.
+      * simpl. rewrite H. rewrite mul_x_x. reflexivity.
+      * simpl. rewrite H. reflexivity.
+      * simpl. rewrite H. reflexivity.
+      * simpl. rewrite <- H. reflexivity.
     + induction t2.
-      { simpl. rewrite H. rewrite mul_comm. rewrite mul_T0_x. reflexivity. }
-      { simpl. rewrite H. rewrite mul_x_x. reflexivity. }
-      { simpl. rewrite H. reflexivity. }
-      { simpl. rewrite H. reflexivity. }
-      { simpl. rewrite <- H. reflexivity. }
+      * simpl. rewrite H. rewrite mul_comm. rewrite mul_T0_x. reflexivity.
+      * simpl. rewrite H. rewrite mul_x_x. reflexivity.
+      * simpl. rewrite H. reflexivity.
+      * simpl. rewrite H. reflexivity.
+      * simpl. rewrite <- H. reflexivity.
   - induction t.
     + induction t2. 
-      { simpl. reflexivity. }
-      { simpl. rewrite H. reflexivity. }
-      { simpl. rewrite <- H. reflexivity. }
-      { simpl. rewrite <- H. reflexivity. }
-      { simpl. rewrite <- H. reflexivity. }
+      * simpl. reflexivity.
+      * simpl. rewrite H. reflexivity.
+      * simpl. rewrite <- H. reflexivity.
+      * simpl. rewrite <- H. reflexivity.
+      * simpl. rewrite <- H. reflexivity.
     + induction t2.
-      { simpl. rewrite H. reflexivity. }
-      { simpl. reflexivity. }
-      { simpl. rewrite H. reflexivity. }
-      { simpl. rewrite H. reflexivity. }
-      { simpl. rewrite <- H. reflexivity. }
+      * simpl. rewrite H. reflexivity.
+      * simpl. reflexivity.
+      * simpl. rewrite H. reflexivity.
+      * simpl. rewrite H. reflexivity.
+      * simpl. rewrite <- H. reflexivity.
     + induction t2.
-      { simpl. rewrite H. reflexivity. }
-      { simpl. rewrite H. reflexivity. }
-      { simpl. rewrite H. reflexivity. }
-      { simpl. rewrite H. reflexivity. }
-      { simpl. rewrite <- H. reflexivity. }
+      * simpl. rewrite H. reflexivity.
+      * simpl. rewrite H. reflexivity.
+      * simpl. rewrite H. reflexivity.
+      * simpl. rewrite H. reflexivity.
+      * simpl. rewrite <- H. reflexivity.
     + induction t2.
-      { simpl. rewrite H. reflexivity. }
-      { simpl. rewrite H. reflexivity. }
-      { simpl. rewrite H. reflexivity. }
-      { simpl. rewrite H. reflexivity. }
-      { simpl. rewrite <- H. reflexivity. }
+      * simpl. rewrite H. reflexivity.
+      * simpl. rewrite H. reflexivity.
+      * simpl. rewrite H. reflexivity.
+      * simpl. rewrite H. reflexivity.
+      * simpl. rewrite <- H. reflexivity.
     + induction t2.
-      { simpl. rewrite H. reflexivity. }
-      { simpl. rewrite H. reflexivity. }
-      { simpl. rewrite H. reflexivity. }
-      { simpl. rewrite H. reflexivity. }
-      { simpl. rewrite <- H. reflexivity. }
+      * simpl. rewrite H. reflexivity.
+      * simpl. rewrite H. reflexivity.
+      * simpl. rewrite H. reflexivity.
+      * simpl. rewrite H. reflexivity.
+      * simpl. rewrite <- H. reflexivity.
   - induction t.
     + induction t2. 
-      { simpl. reflexivity. }
-      { simpl. rewrite H. reflexivity. }
-      { simpl. rewrite <- H. reflexivity. }
-      { simpl. rewrite <- H. reflexivity. }
-      { simpl. rewrite <- H. reflexivity. }
+      * simpl. reflexivity.
+      * simpl. rewrite H. reflexivity.
+      * simpl. rewrite <- H. reflexivity.
+      * simpl. rewrite <- H. reflexivity.
+      * simpl. rewrite <- H. reflexivity.
     + induction t2.
-      { simpl. rewrite H. reflexivity. }
-      { simpl. reflexivity. }
-      { simpl. rewrite H. reflexivity. }
-      { simpl. rewrite H. reflexivity. }
-      { simpl. rewrite <- H. reflexivity. }
+      * simpl. rewrite H. reflexivity.
+      * simpl. reflexivity.
+      * simpl. rewrite H. reflexivity.
+      * simpl. rewrite H. reflexivity.
+      * simpl. rewrite <- H. reflexivity.
     + induction t2.
-      { simpl. rewrite H. reflexivity. }
-      { simpl. rewrite H. reflexivity. }
-      { simpl. rewrite H. reflexivity. }
-      { simpl. rewrite H. reflexivity. }
-      { simpl. rewrite <- H. reflexivity. }
+      * simpl. rewrite H. reflexivity.
+      * simpl. rewrite H. reflexivity.
+      * simpl. rewrite H. reflexivity.
+      * simpl. rewrite H. reflexivity.
+      * simpl. rewrite <- H. reflexivity.
     + induction t2.
-      { simpl. rewrite H. reflexivity. }
-      { simpl. rewrite H. reflexivity. }
-      { simpl. rewrite H. reflexivity. }
-      { simpl. rewrite H. reflexivity. }
-      { simpl. rewrite <- H. reflexivity. }
+      * simpl. rewrite H. reflexivity.
+      * simpl. rewrite H. reflexivity.
+      * simpl. rewrite H. reflexivity.
+      * simpl. rewrite H. reflexivity.
+      * simpl. rewrite <- H. reflexivity.
     + induction t2.
-      { simpl. rewrite H. reflexivity. }
-      { simpl. rewrite H. reflexivity. }
-      { simpl. rewrite H. reflexivity. }
-      { simpl. rewrite H. reflexivity. }
-      { simpl. rewrite <- H. reflexivity. }
+      * simpl. rewrite H. reflexivity.
+      * simpl. rewrite H. reflexivity.
+      * simpl. rewrite H. reflexivity.
+      * simpl. rewrite H. reflexivity.
+      * simpl. rewrite <- H. reflexivity.
   - induction t.
     + induction t2. 
-      { simpl. reflexivity. }
-      { simpl. rewrite H. reflexivity. }
-      { simpl. rewrite <- H. reflexivity. }
-      { simpl. rewrite <- H. reflexivity. }
-      { simpl. rewrite <- H. reflexivity. }
+      * simpl. reflexivity.
+      * simpl. rewrite H. reflexivity.
+      * simpl. rewrite <- H. reflexivity.
+      * simpl. rewrite <- H. reflexivity.
+      * simpl. rewrite <- H. reflexivity.
     + induction t2.
-      { simpl. rewrite H. reflexivity. }
-      { simpl. reflexivity. }
-      { simpl. rewrite H. reflexivity. }
-      { simpl. rewrite H. reflexivity. }
-      { simpl. rewrite <- H. reflexivity. }
+      * simpl. rewrite H. reflexivity.
+      * simpl. reflexivity.
+      * simpl. rewrite H. reflexivity.
+      * simpl. rewrite H. reflexivity.
+      * simpl. rewrite <- H. reflexivity.
     + induction t2.
-      { simpl. rewrite H. reflexivity. }
-      { simpl. rewrite H. reflexivity. }
-      { simpl. rewrite H. reflexivity. }
-      { simpl. rewrite H. reflexivity. }
-      { simpl. rewrite <- H. reflexivity. }
+      * simpl. rewrite H. reflexivity.
+      * simpl. rewrite H. reflexivity.
+      * simpl. rewrite H. reflexivity.
+      * simpl. rewrite H. reflexivity.
+      * simpl. rewrite <- H. reflexivity.
     + induction t2.
-      { simpl. rewrite H. reflexivity. }
-      { simpl. rewrite H. reflexivity. }
-      { simpl. rewrite H. reflexivity. }
-      { simpl. rewrite H. reflexivity. }
-      { simpl. rewrite <- H. reflexivity. }
+      * simpl. rewrite H. reflexivity.
+      * simpl. rewrite H. reflexivity.
+      * simpl. rewrite H. reflexivity.
+      * simpl. rewrite H. reflexivity.
+      * simpl. rewrite <- H. reflexivity.
     + induction t2.
-      { simpl. rewrite H. reflexivity. }
-      { simpl. rewrite H. reflexivity. }
-      { simpl. rewrite H. reflexivity. }
-      { simpl. rewrite H. reflexivity. }
-      { simpl. rewrite <- H. reflexivity. }
+      * simpl. rewrite H. reflexivity.
+      * simpl. rewrite H. reflexivity.
+      * simpl. rewrite H. reflexivity.
+      * simpl. rewrite H. reflexivity.
+      * simpl. rewrite <- H. reflexivity.
 Qed.
 
-(** Being able to simplify a term can be a usefool tool. Being able to use
-the simplified version of the term as the equivalent version of the original term
-can also be useful since many of our functions simplify the term first.
+(** Being able to simplify a term can be a usefool tool. Being able to use the
+    simplified version of the term as the equivalent version of the original
+    term can also be useful since many of our functions simplify the term first.
+    *)
 
-**)
-
-Lemma simplify_eqv :
- forall (t : term),
- simplify t == t.
+Lemma simplify_eqv : forall (t : term),
+  simplify t == t.
 Proof.
- intros. induction t.
- - simpl. reflexivity.
- - simpl. reflexivity.
- - simpl. reflexivity.
- - simpl. pose proof pos_left_sum_compat. specialize (H t1 (simplify t1) (simplify t2)).
-   symmetry in IHt1. specialize (H IHt1). rewrite H.
-  pose proof pos_right_sum_compat. specialize (H0 (simplify t2) t1 t2).
-  specialize (H0 IHt2). symmetry in H0. rewrite H0.
-  induction t1.
-  + induction t2.
-    { simpl. rewrite sum_x_x. reflexivity. }
-    { simpl. rewrite sum_id. reflexivity. }
-    { simpl. reflexivity. }
-    { simpl. reflexivity. }
-    { simpl. reflexivity. }
-  + induction t2.
-    { simpl. rewrite sum_id_sym. reflexivity. }
-    { simpl. rewrite sum_x_x. reflexivity.  } 
-    { simpl. reflexivity. }
-    { simpl. reflexivity. }
-    { simpl. reflexivity.  } 
-  + simpl. reflexivity.
-  + simpl. reflexivity.
-  + simpl. reflexivity.
- - simpl. pose proof pos_left_mul_compat. specialize (H t1 (simplify t1) (simplify t2)).
-   symmetry in IHt1. specialize (H IHt1). rewrite H.
-  pose proof pos_right_mul_compat. specialize (H0 (simplify t2) t1 t2).
-  specialize (H0 IHt2). symmetry in H0. rewrite H0.
-  induction t1.
-  + induction t2.
-    { simpl. rewrite mul_x_x. reflexivity. }
-    { simpl. rewrite mul_T0_x.  reflexivity. }
-    { simpl. reflexivity. }
-    { simpl. reflexivity. }
-    { simpl. reflexivity. }
-  + induction t2.
-    { simpl. rewrite mul_T0_x_sym. reflexivity. }
-    { simpl. rewrite mul_x_x. reflexivity.  } 
-    { simpl. reflexivity. }
-    { simpl. reflexivity. }
-    { simpl. reflexivity.  } 
-  + simpl. reflexivity.
-  + simpl. reflexivity.
-  + simpl. reflexivity.
+  intros. induction t.
+  - simpl. reflexivity.
+  - simpl. reflexivity.
+  - simpl. reflexivity.
+  - simpl. pose proof pos_left_sum_compat.
+    specialize (H t1 (simplify t1) (simplify t2)).
+    symmetry in IHt1. specialize (H IHt1). rewrite H.
+    pose proof pos_right_sum_compat. specialize (H0 (simplify t2) t1 t2).
+    specialize (H0 IHt2). symmetry in H0. rewrite H0.
+    induction t1.
+    + induction t2.
+      * simpl. rewrite sum_x_x. reflexivity.
+      * simpl. rewrite sum_id. reflexivity.
+      * simpl. reflexivity.
+      * simpl. reflexivity.
+      * simpl. reflexivity.
+    + induction t2.
+      * simpl. rewrite sum_id_sym. reflexivity.
+      * simpl. rewrite sum_x_x. reflexivity.  
+      * simpl. reflexivity.
+      * simpl. reflexivity.
+      * simpl. reflexivity.  
+    + simpl. reflexivity.
+    + simpl. reflexivity.
+    + simpl. reflexivity.
+  - simpl. pose proof pos_left_mul_compat.
+    specialize (H t1 (simplify t1) (simplify t2)).
+    symmetry in IHt1. specialize (H IHt1). rewrite H.
+    pose proof pos_right_mul_compat. specialize (H0 (simplify t2) t1 t2).
+    specialize (H0 IHt2). symmetry in H0. rewrite H0.
+    induction t1.
+    + induction t2.
+      * simpl. rewrite mul_x_x. reflexivity.
+      * simpl. rewrite mul_T0_x.  reflexivity.
+      * simpl. reflexivity.
+      * simpl. reflexivity.
+      * simpl. reflexivity.
+    + induction t2.
+      * simpl. rewrite mul_T0_x_sym. reflexivity.
+      * simpl. rewrite mul_x_x. reflexivity.  
+      * simpl. reflexivity.
+      * simpl. reflexivity.
+      * simpl. reflexivity.  
+    + simpl. reflexivity.
+    + simpl. reflexivity.
+    + simpl. reflexivity.
 Qed.
-  
+
